theories/SetModel/HO_acc.v
@@ -8,14 +8,14 @@ Definition ctxExt2 (n : nat) (Γ : ZFSet) (A : ZFSet -> ZFSet) : ZFSet :=
 (* Accessibility predicate *)
 
 Definition accTy_HO (A R a : ZFSet -> ZFSet) : ZFSet -> ZFSet :=
-  fun γ => prop (acc (A γ) (fun x y => ∅ ∈ R ⟨ ⟨ γ ; y ⟩ ; x ⟩) (a γ)).
+  fun γ => subsingl (acc (A γ) (fun x y => ∅ ∈ R ⟨ ⟨ γ ; y ⟩ ; x ⟩) (a γ)).
 
 Lemma accTy_HO_typing {n : nat} {Γ : ZFSet} {A R a : ZFSet -> ZFSet}
   (HA : ∀ γ ∈ Γ, A γ ∈ 𝕌 n) (HR : ∀ γaa ∈ ctxExt2 n Γ A, R γaa ∈ Ω)
   (Ha : ∀ γ ∈ Γ, a γ ∈ 𝕌el n (A γ)) :
   ∀ γ ∈ Γ, accTy_HO A R a γ ∈ Ω.
 Proof.
-  intros γ Hγ. unfold accTy_HO. apply prop_typing.
+  intros γ Hγ. unfold accTy_HO. apply subsingl_typing.
 Qed.
 
 (* Eliminator of accessibility *)
