theories/SetModel/HO_forall.v
@@ -5,13 +5,13 @@ Require Import HO HO_prop HO_univ HO_box.
 (* Proof-irrelevant pi types *)
 
 Definition forallTy_HO (n : nat) (A : ZFSet -> ZFSet) (B : ZFSet -> ZFSet) : ZFSet -> ZFSet :=
-  fun γ => prop (∀ a ∈ 𝕌el n (A γ), ∅ ∈ B ⟨ γ ; a ⟩).
+  fun γ => subsingl (∀ a ∈ 𝕌el n (A γ), ∅ ∈ B ⟨ γ ; a ⟩).
 
 Lemma forallTy_HO_typing {n : nat} {Γ : ZFSet} {A : ZFSet -> ZFSet} {B : ZFSet -> ZFSet}
   (HA : ∀ γ ∈ Γ, A γ ∈ 𝕌 n) (HB : ∀ γa ∈ ctxExt n Γ A, B γa ∈ Ω) :
   ∀ γ ∈ Γ, forallTy_HO n A B γ ∈ Ω.
 Proof.
-  intros γ Hγ. unfold forallTy_HO. apply prop_typing.
+  intros γ Hγ. unfold forallTy_HO. apply subsingl_typing.
 Qed.
 
 Lemma forallTy_HO_typing' {n : nat} {Γ : ZFSet} {A : ZFSet -> ZFSet} {B : ZFSet -> ZFSet}
@@ -30,7 +30,7 @@ Lemma ilamTm_HO_typing (n : nat) {Γ : ZFSet} {A B : ZFSet -> ZFSet}
   ∀ γ ∈ Γ, ∅ ∈ forallTy_HO n A B γ.
 Proof.
   intros γ Hγ. cbn. unfold forallTy_HO.
-  apply prop_true_iff. intros a Ha. assert (⟨ γ ; a ⟩ ∈ ctxExt n Γ A) as Hγa.
+  apply subsingl_true_iff. intros a Ha. assert (⟨ γ ; a ⟩ ∈ ctxExt n Γ A) as Hγa.
   { apply setMkSigma_typing ; try assumption. intros γ' Hγ'. apply 𝕌el_typing. now apply HA. }
   specialize (Ht _ Hγa). cbn in Ht. specialize (HB _ Hγa). cbn in HB.
   refine (proof_irr' HB _ Ht).
@@ -44,7 +44,7 @@ Lemma iappTm_HO_typing (n : nat) {Γ : ZFSet} {A B u : ZFSet -> ZFSet}
   ∀ γ ∈ Γ, ∅ ∈ B ⟨ γ ; u γ ⟩.
 Proof.
   intros γ Hγ. cbn. 
-  specialize (Ht _ Hγ). cbn in Ht. unfold forallTy_HO in Ht. apply prop_true_if in Ht.
+  specialize (Ht _ Hγ). cbn in Ht. unfold forallTy_HO in Ht. apply subsingl_true_if in Ht.
   apply Ht. now apply Hu.
 Qed.
 
@@ -54,19 +54,19 @@ Definition implTy_HO' (Γ : ZFSet) (P : ZFSet -> ZFSet) (Q : ZFSet -> ZFSet) : Z
   forallTy_HO 0 (boxTy_HO P) (fun γa => Q (ctx_wk 0 Γ (boxTy_HO P) γa)).
 
 Definition implTy_HO (P : ZFSet -> ZFSet) (Q : ZFSet -> ZFSet) : ZFSet -> ZFSet :=
-  fun γ => prop (P γ ⊂ Q γ).
+  fun γ => subsingl (P γ ⊂ Q γ).
 
 Lemma implTy_HO_typing {Γ : ZFSet} {P : ZFSet -> ZFSet} {Q : ZFSet -> ZFSet}
   (HP : ∀ γ ∈ Γ, P γ ∈ Ω) (HQ : ∀ γ ∈ Γ, Q γ ∈ Ω) : ∀ γ ∈ Γ, implTy_HO P Q γ ∈ Ω.
 Proof.
-  intros. now apply prop_typing.
+  intros. now apply subsingl_typing.
 Qed.
 
 Lemma implTy_HO_eq_implTy_HO' {Γ : ZFSet} {P : ZFSet -> ZFSet} {Q : ZFSet -> ZFSet}
   (HP : ∀ γ ∈ Γ, P γ ∈ Ω) (HQ : ∀ γ ∈ Γ, Q γ ∈ Ω) : ∀ γ ∈ Γ, implTy_HO P Q γ ≡ implTy_HO' Γ P Q γ.
 Proof.
   intros γ Hγ. unfold implTy_HO. unfold implTy_HO'. unfold forallTy_HO.
-  apply (fstS prop_ext). split.
+  apply (fstS subsingl_ext). split.
   - intros H x Hx. refine (transpS (fun X => ∅ ∈ Q X) (sym _) _).
     { apply ctxExtβ1 ; try assumption. intros γ' Hγ'. now apply (boxTy_HO_typing (Γ := Γ)). }
     apply H. eapply proof_irr'. now apply HP. exact (transpS (fun X => _ ∈ X) (el_boxTy HP γ Hγ) Hx).
