theories/SetModel/HO_obseq.v
@@ -6,13 +6,21 @@ Require Import HO HO_prop HO_univ HO_forall HO_nat HO_pi.
 (* Observational equality *)
 
 Definition eqTy_HO (A t u : ZFSet -> ZFSet) : ZFSet -> ZFSet :=
-  fun γ => prop (t γ ≡ u γ).
+  fun γ => subsingl (t γ ≡ u γ).
 
 Lemma eqTy_HO_typing {n : nat} {Γ : ZFSet} {A t u : ZFSet -> ZFSet}
   (HA : ∀ γ ∈ Γ, A γ ∈ 𝕌 n) (Ht : ∀ γ ∈ Γ, t γ ∈ 𝕌el n (A γ)) (Hu : ∀ γ ∈ Γ, u γ ∈ 𝕌el n (A γ)) :
   ∀ γ ∈ Γ, eqTy_HO A t u γ ∈ Ω.
 Proof.
-  intros γ Hγ. cbn. apply prop_typing.
+  intros γ Hγ. cbn. apply subsingl_typing.
+Qed.
+
+Lemma eqTy_HO_typing' {n : nat} {Γ : ZFSet} {A t u : ZFSet -> ZFSet}
+  (HA : ∀ γ ∈ Γ, A γ ∈ 𝕌 n) (Ht : ∀ γ ∈ Γ, t γ ∈ 𝕌el n (A γ)) (Hu : ∀ γ ∈ Γ, u γ ∈ 𝕌el n (A γ)) :
+  ∀ γ ∈ Γ, eqTy_HO A t u γ ∈ 𝕌el 0 (propTy_HO γ).
+Proof.
+  intros γ Hγ. refine (transpS (fun X => _ ∈ X) (sym _) (eqTy_HO_typing HA Ht Hu γ Hγ)).
+  now apply el_propTy.  
 Qed.
 
 (* Reflexivity *)
@@ -23,7 +31,7 @@ Lemma reflTm_HO_typing {n : nat} {Γ : ZFSet} {A t : ZFSet -> ZFSet}
   (HA : ∀ γ ∈ Γ, A γ ∈ 𝕌 n) (Ht : ∀ γ ∈ Γ, t γ ∈ 𝕌el n (A γ)) :
   ∀ γ ∈ Γ, reflTm_HO A t γ ∈ eqTy_HO A t t γ.
 Proof.
-  intros γ Hγ. unfold reflTm_HO. apply prop_true_iff. reflexivity.
+  intros γ Hγ. unfold reflTm_HO. apply subsingl_true_iff. reflexivity.
 Qed.
 
 (* J eliminator *)
@@ -36,7 +44,7 @@ Lemma eqindTm_HO_typing {n : nat} {Γ : ZFSet} {A t P p u e : ZFSet -> ZFSet}
   ∀ γ ∈ Γ, eqindTm_HO A t P p u e γ ∈ P ⟨ γ ; u γ ⟩.
 Proof.
   intros γ Hγ. unfold eqindTm_HO. specialize (He γ Hγ). unfold eqTy_HO in He.
-  apply prop_true_if in He. refine (transpS (fun X => ∅ ∈ P ⟨ γ ; X ⟩) He _). specialize (Ht γ Hγ).
+  apply subsingl_true_if in He. refine (transpS (fun X => ∅ ∈ P ⟨ γ ; X ⟩) He _). specialize (Ht γ Hγ).
   assert (⟨ γ ; t γ ⟩ ∈ ctxExt n Γ A) as Hγt.
   { apply setMkSigma_typing ; try assumption. clear γ Ht He Hγ. intros γ Hγ. apply 𝕌el_typing. now apply HA. }
   specialize (HP ⟨ γ ; t γ ⟩ Hγt). cbn in HP. eapply (proof_irr' HP). now apply Hp.
@@ -51,7 +59,7 @@ Lemma castTm_HO_typing {n : nat} {Γ : ZFSet} {A B e t : ZFSet -> ZFSet}
   (Ht : ∀ γ ∈ Γ, t γ ∈ 𝕌el n (A γ)) : ∀ γ ∈ Γ, castTm_HO A B e t γ ∈ 𝕌el n (B γ).
 Proof.
   intros γ Hγ. unfold castTm_HO. specialize (He γ Hγ). unfold eqTy_HO in He.
-  apply prop_true_if in He. refine (transpS (fun X => t γ ∈ 𝕌el n X) He _).
+  apply subsingl_true_if in He. refine (transpS (fun X => t γ ∈ 𝕌el n X) He _).
   now apply Ht.
 Qed.
 
@@ -74,13 +82,13 @@ Lemma funextTm_HO_typing {nA nB : nat} {Γ : ZFSet} {A B f g e : ZFSet -> ZFSet}
                        (appTm_HO nA nB (fun γa => A (ctx_wk nA Γ A γa)) (fun γa => g (ctx_wk nA Γ A γa)) (ctx_var0 nA Γ A)) γa) :
   ∀ γ ∈ Γ, funextTm_HO A B f g e γ ∈ eqTy_HO (piTy_HO nA nB A B) f g γ.
 Proof.
-  intros γ Hγ. unfold funextTm_HO. unfold eqTy_HO. apply prop_true_iff.
+  intros γ Hγ. unfold funextTm_HO. unfold eqTy_HO. apply subsingl_true_iff.
   apply (setArr_funext (A := 𝕌el nA (A γ)) (B := 𝕍 (max nA nB))).
   - pose proof (transpS (fun X => f γ ∈ X) (el_piTy HA HB Hγ) (Hf γ Hγ)) as H. apply ZFincomp in H. now destruct H.
   - pose proof (transpS (fun X => g γ ∈ X) (el_piTy HA HB Hγ) (Hg γ Hγ)) as H. apply ZFincomp in H. now destruct H.
   - intros a Ha. assert (⟨ γ ; a ⟩ ∈ ctxExt nA Γ A) as Hγa.
     { apply setMkSigma_typing ; try assumption. intros γ' Hγ'. apply 𝕌el_typing. now apply HA. }
-    specialize (He _ Hγa). apply prop_true_if in He. refine (trans (sym _) (trans He _)).
+    specialize (He _ Hγa). apply subsingl_true_if in He. refine (trans (sym _) (trans He _)).
     + refine (fequal2 (fun X Y => setAppArr (𝕌el nA (A X)) (𝕍 (max nA nB)) (f X) Y) _ _).
       * now apply ctxExtβ1.
       * now apply ctxExtβ2.
@@ -97,7 +105,7 @@ Lemma propextTm_HO_typing {Γ : ZFSet} {P Q e f : ZFSet -> ZFSet}
   (HP : ∀ γ ∈ Γ, P γ ∈ Ω) (HQ : ∀ γ ∈ Γ, Q γ ∈ Ω) (He : ∀ γ ∈ Γ, e γ ∈ implTy_HO P Q γ)
   (Hf : ∀ γ ∈ Γ, f γ ∈ implTy_HO Q P γ) : ∀ γ ∈ Γ, propextTm_HO P Q e f γ ∈ eqTy_HO propTy_HO P Q γ.
 Proof.
-  intros γ Hγ. cbn. unfold propextTm_HO. unfold eqTy_HO. apply prop_true_iff. apply ZFext.
+  intros γ Hγ. cbn. unfold propextTm_HO. unfold eqTy_HO. apply subsingl_true_iff. apply ZFext.
   - unfold implTy_HO in He. specialize (He γ Hγ). apply ZFincomp in He. now destruct He.
   - unfold implTy_HO in Hf. specialize (Hf γ Hγ). apply ZFincomp in Hf. now destruct Hf.
 Qed.
@@ -112,9 +120,9 @@ Lemma piinj1Tm_HO_typing {nA nB : nat} {Γ : ZFSet} {A A' B B' e : ZFSet -> ZFSe
   (He : ∀ γ ∈ Γ, e γ ∈ eqTy_HO (univTy_HO (max nA nB)) (piTy_HO nA nB A B) (piTy_HO nA nB A' B') γ)
   : ∀ γ ∈ Γ, piinj1Tm_HO A A' B B' e γ ∈ eqTy_HO (univTy_HO (max nA nB)) A' A γ.
 Proof.
-  intros γ Hγ. cbn. unfold eqTy_HO. unfold piinj1Tm_HO. apply prop_true_iff. apply sym.
+  intros γ Hγ. cbn. unfold eqTy_HO. unfold piinj1Tm_HO. apply subsingl_true_iff. apply sym.
   apply (piTy_HO_inj_dom HA HB HA' HB' Hγ). specialize (He γ Hγ). unfold eqTy_HO in He.
-  now apply prop_true_if in He.
+  now apply subsingl_true_if in He.
 Qed.
 
 Definition piinj2Tm_HO (A A' B B' e a : ZFSet -> ZFSet) : ZFSet -> ZFSet := fun _ => ∅.
@@ -126,9 +134,9 @@ Lemma piinj2Tm_HO_typing {nA nB : nat} {Γ : ZFSet} {A A' B B' e a : ZFSet -> ZF
   (Ha : ∀ γ ∈ Γ, a γ ∈ 𝕌el nA (A' γ)) (a0 := castTm_HO A' A (piinj1Tm_HO A A' B B' e) a)
   : ∀ γ ∈ Γ, piinj2Tm_HO A A' B B' e a γ ∈ eqTy_HO (univTy_HO (max nA nB)) (fun γ => B ⟨ γ ; a0 γ ⟩) (fun γ => B' ⟨ γ ; a γ ⟩) γ.
 Proof.
-  intros γ Hγ. cbn. unfold piinj2Tm_HO. unfold eqTy_HO. apply prop_true_iff.
+  intros γ Hγ. cbn. unfold piinj2Tm_HO. unfold eqTy_HO. apply subsingl_true_iff.
   unfold castTm_HO in a0. unfold a0. clear a0. specialize (He γ Hγ). unfold eqTy_HO in He.
-  apply prop_true_if in He. assert (a γ ∈ 𝕌el nA (A γ)).
+  apply subsingl_true_if in He. assert (a γ ∈ 𝕌el nA (A γ)).
   { refine (transpS (fun X => a γ ∈ 𝕌el nA X) _ (Ha γ Hγ)). apply sym.
     now apply (piTy_HO_inj_dom HA HB HA' HB' Hγ). }
   apply (piTy_HO_inj_cod HA HB HA' HB' Hγ He H).
@@ -153,7 +161,7 @@ Lemma castTm_HO_pi {nA nB : nat} {Γ : ZFSet} {A A' B B' e f : ZFSet -> ZFSet}
 Proof.
   intros γ Hγ. unfold castTm_HO in *. unfold t4. unfold t3. unfold t2. unfold t1. unfold Au.
   clear t1 t2 t3 t4. unfold lamTm_HO. unfold appTm_HO.
-  specialize (He γ Hγ). unfold eqTy_HO in He. apply prop_true_if in He.
+  specialize (He γ Hγ). unfold eqTy_HO in He. apply subsingl_true_if in He.
   assert (A γ ≡ A' γ) as HAA'. { now apply (piTy_HO_inj_dom HA HB HA' HB' Hγ). }
   assert (f γ ∈ setPi (max nA nB) (𝕌el nA (A' γ)) (fun a => 𝕌el nB (B' ⟨ γ ; a ⟩))) as Hf'.
   { refine (transpS (fun X => f γ ∈ X) (el_piTy HA' HB' Hγ) _).
@@ -183,7 +191,7 @@ Lemma nat_neq_pi {nA nB : nat} {Γ : ZFSet} {A B e : ZFSet -> ZFSet}
   (He : ∀ γ ∈ ⋆, e γ ∈ eqTy_HO (univTy_HO (max nA nB)) natTy_HO (piTy_HO nA nB A B) γ) : FalseS.
 Proof.
   assert (∅ ∈ ⋆) as H. { now apply inSetSingl. }
-  specialize (He _ H). cbn in He. unfold eqTy_HO in He. apply prop_true_if in He.
+  specialize (He _ H). cbn in He. unfold eqTy_HO in He. apply subsingl_true_if in He.
   assert (ZFzero ≡ ZFone).
   { refine (trans (sym _) (trans (fequal (𝕌hd (max nA nB)) He) _)).
     - now apply hd_natTy.
