theories/SetModel/BasicAST.v
@@ -1,0 +1,9 @@
+From Stdlib Require Import Utf8 String.
+
+Set Primitive Projections.
+
+(** Universe level *)
+Inductive level := 
+| ty (n : nat) | prop.
+
+Definition aref := nat.
