theories/SetModel/HO_false.v
@@ -4,11 +4,11 @@ Require Import HO HO_prop.
 
 (* False proposition *)
 
-Definition falseTy_HO : ZFSet -> ZFSet := fun γ => prop FalseS.
+Definition falseTy_HO : ZFSet -> ZFSet := fun γ => subsingl FalseS.
 
 Lemma falseTy_HO_typing (Γ : ZFSet) : ∀ γ ∈ Γ, falseTy_HO γ ∈ Ω.
 Proof.
-  intros. cbn. apply prop_typing.
+  intros. cbn. apply subsingl_typing.
 Qed.
 
 (* Eliminator of False *)
@@ -19,5 +19,5 @@ Lemma emptyrecTm_HO_typing {n : nat} {Γ : ZFSet} {A H : ZFSet -> ZFSet}
   (HA : ∀ γ ∈ Γ, A γ ∈ 𝕌 n) (HH : ∀ γ ∈ Γ, H γ ∈ falseTy_HO γ) :
   ∀ γ ∈ Γ, emptyrecTm_HO A H ∈ 𝕌el n (A γ).
 Proof.
-  intros γ Hγ. specialize (HH γ Hγ). cbn in HH. apply prop_true_if in HH. destruct HH.
+  intros γ Hγ. specialize (HH γ Hγ). cbn in HH. apply subsingl_true_if in HH. destruct HH.
 Qed.
