theories/SetModel/Typing.v
@@ -1,0 +1,529 @@
+(** * Typing *)
+
+From Stdlib Require Import Utf8 List Arith Bool.
+From TypedConfluence
+Require Import core unscoped AST SubstNotations RAsimpl AST_rasimpl.
+From TypedConfluence Require Import Util BasicAST Contexts. (*  Env Inst. *)
+From Stdlib Require Import Setoid Morphisms Relation_Definitions.
+
+Import ListNotations.
+Import CombineNotations.
+
+Set Default Goal Selector "!".
+
+Open Scope subst_scope.
+
+Definition ax (l : level) :=
+  match l with
+  | prop => 0
+  | ty i => S i
+  end.
+
+Definition ru l j :=
+    match l with
+    | prop => j
+    | ty i => max i j
+    end.
+
+
+
+Definition Ax (l : level) : level :=
+  ty (ax l).
+
+Definition Ru (l1 l2 : level) : level :=
+  match l2 with
+  | prop => prop
+  | ty j => ty (ru l1 j)
+  end.
+
+
+Parameter assm_sig : list term.
+
+Reserved Notation "Γ ⊢< l > t : T" (at level 50, l, t, T at next level).
+Reserved Notation "Γ ⊢< l > t ≡ u : T" (at level 50, l, t, u, T at next level).
+Reserved Notation "⊢ Γ" (at level 50).
+
+Inductive typing : ctx -> level -> term → term → Prop :=
+
+| type_var :
+    ∀ Γ x l A,
+      ⊢ Γ ->
+      nth_error Γ x = Some (l , A) →
+      (Γ ⊢< l > (var x) : ((plus (S x)) ⋅ A))
+
+| type_sort :
+    ∀ Γ l,
+      ⊢ Γ ->
+      Γ ⊢< Ax (Ax l) > Sort l : Sort (Ax l)
+
+| type_assm :
+    ∀ Γ c A,
+      ⊢ Γ ->
+      nth_error assm_sig c = Some A ->
+      ∙ ⊢< Ax prop > A : Sort prop ->
+      Γ ⊢< prop > assm c : A
+
+| type_pi :
+    ∀ Γ i j A B,
+      Γ ⊢< Ax i > A : Sort i →
+      Γ ,, (i , A) ⊢< Ax j > B : Sort j →
+      Γ ⊢< Ax (Ru i j) > Pi i j A B : Sort (Ru i j)
+
+
+| type_lam :
+    ∀ Γ i j A B t,
+      Γ ⊢< Ax i > A : Sort i →
+      Γ ,, (i , A) ⊢< Ax j > B : Sort j →
+      Γ ,, (i , A) ⊢< j > t : B →
+      Γ ⊢< Ru i j > lam i j A B t : Pi i j A B
+
+| type_app :
+    ∀ Γ i j A B t u,
+      Γ ⊢< Ax i > A : Sort i →
+      Γ ,, (i , A) ⊢< Ax j > B : Sort j →
+      Γ ⊢< Ru i j > t : Pi i j A B →
+      Γ ⊢< i > u : A →
+      Γ ⊢< j > app i j A B  t u : B <[ u .. ]
+
+| type_nat :
+    ∀ Γ,
+      ⊢ Γ ->
+      Γ ⊢< ty 1 > Nat : Sort (ty 0)
+
+| type_zero :
+    ∀ Γ,
+      ⊢ Γ ->
+      Γ ⊢< ty 0 > zero : Nat
+
+| type_succ :
+    ∀ Γ t,
+      Γ ⊢< ty 0 > t : Nat ->
+      Γ ⊢< ty 0 > succ t : Nat
+
+| type_rec :
+    ∀ Γ l P p_zero p_succ t,
+      Γ ,, (ty 0 , Nat) ⊢< Ax l > P : Sort l ->
+      Γ ⊢< l > p_zero : P <[ zero .. ] ->
+      Γ ,, (ty 0 , Nat) ,, (l , P) ⊢< l > p_succ : P <[ (succ (var 1)) .: (shift >> (shift >> var)) ] ->
+      Γ ⊢< ty 0 > t : Nat ->
+      Γ ⊢< l > rec l P p_zero p_succ t : P <[ t .. ]
+
+| type_acc :
+    ∀ Γ i A R a,
+    Γ ⊢< Ax i > A : Sort i ->
+    Γ ,, (i, A) ,, (i, S ⋅ A) ⊢< Ax prop > R : Sort prop ->
+    Γ ⊢< i > a : A ->
+    Γ ⊢< Ax prop > acc i A R a : Sort prop
+
+| type_accin :
+    ∀ Γ i A R a p,
+    Γ ⊢< Ax i > A : Sort i ->
+    Γ ,, (i, A) ,, (i, S ⋅ A) ⊢< Ax prop > R : Sort prop ->
+    Γ ⊢< i > a : A ->
+    let A_wk := (S >> S) ⋅ A in
+    let R_wk := (up_ren (up_ren (S >> S))) ⋅ R in
+    let acc_wk := acc i A_wk R_wk (var 1)  in
+    let R' := R <[(S ⋅ a) .: (var 0 .: (S >> var))] in
+    Γ ⊢< prop > p : Pi i prop A (Pi prop prop R' acc_wk) ->
+    Γ ⊢< prop > accin i A R a p : acc i A R a
+
+| type_accinv :
+    ∀ Γ i A R a p b r,
+    Γ ⊢< Ax i > A : Sort i ->
+    Γ ,, (i, A) ,, (i, S ⋅ A) ⊢< Ax prop > R : Sort prop ->
+    Γ ⊢< i > a : A ->
+    Γ ⊢< prop > p : acc i A R a ->
+    Γ ⊢< i > b : A ->
+    Γ ⊢< prop > r : R <[a.:b..] ->
+    Γ ⊢< prop > accinv i A R a p b r : acc i A R b
+
+| type_accel :
+    ∀ Γ i l A R a q P p,
+    Γ ⊢< Ax i > A : Sort i ->
+    Γ ,, (i, A) ,, (i, S ⋅ A) ⊢< Ax prop > R : Sort prop ->
+    Γ ,, (i, A) ⊢< Ax l > P : Sort l ->
+    let R' := R <[var 1 .: (var 0 .: (S >> S >> var))] in
+    let P' := P <[var 1 .: (S >> S >> S >> var)] in
+    let B := Pi i l (S ⋅ A) (Pi prop l R' P') in
+    let P'' := P <[var 1.: (S >> (S >> var))] in
+    Γ ,, (i, A) ,, (Ru i l, B) ⊢< l > p : P'' ->
+    Γ ⊢< i > a : A ->
+    Γ ⊢< prop > q : acc i A R a ->
+    Γ ⊢< l > accel i l A R P p a q : P <[a ..]
+
+| type_obseq :
+    ∀ Γ i A a b,
+    Γ ⊢< Ax i > A : Sort i ->
+    Γ ⊢< i > a : A ->
+    Γ ⊢< i > b : A ->
+    Γ ⊢< Ax prop > obseq i A a b : Sort prop
+
+| type_obsrefl :
+    ∀ l Γ A a,
+      Γ ⊢< Ax l > A : Sort l ->
+      Γ ⊢< l > a : A ->
+      Γ ⊢< prop > obsrefl l A a : obseq l A a a
+
+| type_J :
+    ∀ Γ l A a P p b e,
+      Γ ⊢< Ax l > A : Sort l ->
+      Γ ⊢< l > a : A ->
+      Γ ,, (l , A) ⊢< Ax prop > P : Sort prop ->
+      Γ ⊢< prop > p : P <[a..] ->
+      Γ ⊢< l > b : A ->
+      Γ ⊢< prop > e : obseq l A a b ->
+      Γ ⊢< prop > J l A a P p b e : P <[b..]
+
+| type_cast :
+  ∀ Γ i A B e a,
+    Γ ⊢< Ax i > A : Sort i ->
+    Γ ⊢< Ax i > B : Sort i ->
+    Γ ⊢< prop > e : obseq (Ax i) (Sort i) A B ->
+    Γ ⊢< i > a : A ->
+    Γ ⊢< i > cast i A B e a : B
+
+| type_injpi1 :
+  ∀ Γ i j A1 A2 B1 B2 e,
+    Γ ⊢< Ax i > A1 : Sort i ->
+    Γ ,, (i, A1) ⊢< Ax j > B1 : Sort j ->
+    Γ ⊢< Ax i > A2 : Sort i ->
+    Γ ,, (i, A2) ⊢< Ax j > B2 : Sort j ->
+    Γ ⊢< prop > e : obseq (Ax (Ru i j)) (Sort (Ru i j)) (Pi i j A1 B1) (Pi i j A2 B2) ->
+    Γ ⊢< prop > injpi1 i j A1 A2 B1 B2 e : obseq (Ax i) (Sort i) A2 A1
+
+| type_injpi2 :
+  ∀ Γ i j A1 A2 B1 B2 e a2,
+    Γ ⊢< Ax i > A1 : Sort i ->
+    Γ ,, (i, A1) ⊢< Ax j > B1 : Sort j ->
+    Γ ⊢< Ax i > A2 : Sort i ->
+    Γ ,, (i, A2) ⊢< Ax j > B2 : Sort j ->
+    Γ ⊢< prop > e : obseq (Ax (Ru i j)) (Sort (Ru i j)) (Pi i j A1 B1) (Pi i j A2 B2) ->
+    Γ ⊢< i > a2 : A2 ->
+    let a1 := cast i A2 A1 (injpi1 i j A1 A2 B1 B2 e) a2 in
+    Γ ⊢< prop > injpi2 i j A1 A2 B1 B2 e a2 : obseq (Ax j) (Sort j) (B1<[a1..]) (B2 <[a2..])
+
+| type_conv :
+    ∀ Γ l A B t,
+      Γ ⊢< l > t : A ->
+      Γ ⊢< Ax l > A ≡ B : Sort l ->
+      Γ ⊢< l > t : B
+
+with ctx_typing : ctx -> Prop :=
+| ctx_nil :
+      ⊢ ∙
+
+| ctx_cons :
+    ∀ Γ l A,
+      ⊢ Γ ->
+      Γ ⊢< Ax l > A : Sort l ->
+      ⊢ (Γ ,, (l , A))
+
+with conversion : ctx -> level -> term -> term -> term -> Prop :=
+
+
+| conv_var :
+    ∀ Γ x l A,
+      nth_error Γ x = Some (l , A) →
+      ⊢ Γ ->
+      (Γ ⊢< l > (var x) ≡ (var x) : ((plus (S x)) ⋅ A))
+
+| conv_sort :
+    ∀ Γ l,
+      ⊢ Γ ->
+      Γ ⊢< Ax (Ax l) > Sort l ≡ Sort l : Sort (Ax l)
+
+| conv_assm :
+    ∀ Γ c A,
+      ⊢ Γ ->
+      nth_error assm_sig c = Some A ->
+      ∙ ⊢< Ax prop > A : Sort prop ->
+      Γ ⊢< prop > assm c ≡ assm c : A
+
+
+| conv_pi :
+    ∀ Γ i j A B A' B',
+      Γ ⊢< Ax i > A ≡ A' : Sort i →
+      Γ ,, (i , A) ⊢< Ax j > B ≡ B' : Sort j →
+      Γ ⊢< Ax (Ru i j) > Pi i j A B ≡ Pi i j A' B' : Sort (Ru i j)
+
+| conv_lam :
+    ∀ Γ i j A B t A' B' t',
+      Γ ⊢< Ax i > A ≡ A' : Sort i →
+      Γ ,, (i , A) ⊢< Ax j > B ≡ B': Sort j →
+      Γ ,, (i , A) ⊢< j > t ≡ t' : B →
+      Γ ⊢< Ru i j > lam i j A B t ≡ lam i j A' B' t' : Pi i j A B
+
+| conv_app :
+    ∀ Γ i j A B t u A' B' t' u',
+      Γ ⊢< Ax i > A ≡ A' : Sort i →
+      Γ ,, (i , A) ⊢< Ax j > B ≡ B': Sort j →
+      Γ ⊢< Ru i j > t ≡ t' : Pi i j A B →
+      Γ ⊢< i > u ≡ u' : A →
+      Γ ⊢< j > app i j A B t u ≡ app i j A' B' t' u' : B <[ u .. ]
+
+
+| conv_nat :
+    ∀ Γ,
+      ⊢ Γ ->
+      Γ ⊢< ty 1 > Nat ≡ Nat : Sort (ty 0)
+
+| conv_zero :
+    ∀ Γ,
+      ⊢ Γ ->
+      Γ ⊢< ty 0 > zero ≡ zero : Nat
+
+| conv_succ :
+    ∀ Γ t t',
+      Γ ⊢< ty 0 > t ≡ t' : Nat ->
+      Γ ⊢< ty 0 > succ t ≡ succ t' : Nat
+
+| conv_rec :
+    ∀ Γ l P p_zero p_succ t P' p_zero' p_succ' t',
+      Γ ,, (ty 0 , Nat) ⊢< Ax l > P ≡ P' : Sort l ->
+      Γ ⊢< l > p_zero ≡ p_zero' : P <[ zero .. ] ->
+      Γ ,, (ty 0 , Nat) ,, (l , P) ⊢< l > p_succ ≡ p_succ' : P <[ (succ (var 1)) .: (shift >> (shift >> var)) ] ->
+      Γ ⊢< ty 0 > t ≡ t' : Nat ->
+      Γ ⊢< l > rec l P p_zero p_succ t ≡ rec l P' p_zero' p_succ' t' : P <[ t .. ]
+
+
+| conv_acc :
+    ∀ Γ i A A' R R' a a',
+    Γ ⊢< Ax i > A ≡ A' : Sort i ->
+    Γ ,, (i, A) ,, (i, S ⋅ A) ⊢< Ax prop > R ≡ R' : Sort prop ->
+    Γ ⊢< i > a ≡ a' : A ->
+    Γ ⊢< Ax prop > acc i A R a ≡ acc i A' R' a' : Sort prop
+
+| conv_accin :
+    ∀ Γ i A A' R R' a a' p p',
+    Γ ⊢< Ax i > A ≡ A' : Sort i ->
+    Γ ,, (i, A) ,, (i, S ⋅ A) ⊢< Ax prop > R ≡ R' : Sort prop ->
+    Γ ⊢< i > a ≡ a' : A ->
+    let A_wk := (S >> S) ⋅ A in
+    let R_wk := (up_ren (up_ren (S >> S))) ⋅ R in
+    let acc_wk := acc i A_wk R_wk (var 1)  in
+    let R' := R <[(S ⋅ a) .: (var 0 .: (S >> var))] in
+    Γ ⊢< prop > p ≡ p' : Pi i prop A (Pi prop prop R' acc_wk) ->
+    Γ ⊢< prop > accin i A R a p ≡ accin i A' R' a' p' : acc i A R a
+
+| conv_accinv :
+    ∀ Γ i A A' R R' a a' p p' b b' r r',
+    Γ ⊢< Ax i > A ≡ A' : Sort i ->
+    Γ ,, (i, A) ,, (i, S ⋅ A) ⊢< Ax prop > R ≡ R' : Sort prop ->
+    Γ ⊢< i > a ≡ a' : A ->
+    Γ ⊢< prop > p ≡ p' : acc i A R a ->
+    Γ ⊢< i > b ≡ b' : A ->
+    Γ ⊢< prop > r ≡ r' : R <[a.:b..] ->
+    Γ ⊢< prop > accinv i A R a p b r ≡ accinv i A' R' a' p' b' r' : acc i A R b
+
+| conv_accel :
+    ∀ Γ i l A A' R R' a a' q q' P P' p p',
+    Γ ⊢< Ax i > A ≡ A' : Sort i ->
+    Γ ,, (i, A) ,, (i, S ⋅ A) ⊢< Ax prop > R ≡ R' : Sort prop ->
+    Γ ,, (i, A) ⊢< Ax l > P ≡ P' : Sort l ->
+    let R_ := R <[var 1 .: (var 0 .: (S >> S >> var))] in
+    let P_ := P <[var 1 .: (S >> S >> S >> var)] in
+    let B := Pi i l (S ⋅ A) (Pi prop l R_ P_) in
+    let P'' := P <[var 1.: (S >> (S >> var))] in
+    Γ ,, (i, A) ,, (Ru i l, B) ⊢< l > p ≡ p' : P'' ->
+    Γ ⊢< i > a ≡ a': A ->
+    Γ ⊢< prop > q ≡ q' : acc i A R a ->
+    Γ ⊢< l > accel i l A R P p a q ≡ accel i l A' R' P' p' a' q' : P <[a ..]
+
+
+| conv_obseq :
+    ∀ Γ i A A' a a' b b',
+    Γ ⊢< Ax i > A ≡ A' : Sort i ->
+    Γ ⊢< i > a ≡ a' : A ->
+    Γ ⊢< i > b ≡ b' : A ->
+    Γ ⊢< Ax prop > obseq i A a b ≡ obseq i A' a' b' : Sort prop
+
+| conv_obsrefl :
+  ∀ l Γ A A' a a',
+    Γ ⊢< Ax l > A ≡ A' : Sort l ->
+    Γ ⊢< l > a ≡ a' : A ->
+    Γ ⊢< prop > obsrefl l A a ≡ obsrefl l A' a' : obseq l A a a
+
+| conv_J :
+    ∀ Γ l A A' a a' P P' p p' b b' e e',
+      Γ ⊢< Ax l > A ≡ A' : Sort l ->
+      Γ ⊢< l > a ≡ a' : A ->
+      Γ ,, (l , A) ⊢< Ax prop > P ≡ P' : Sort prop ->
+      Γ ⊢< prop > p ≡ p' : P <[a..] ->
+      Γ ⊢< l > b ≡ b' : A ->
+      Γ ⊢< prop > e ≡ e' : obseq l A a b ->
+      Γ ⊢< prop > J l A a P p b e ≡ J l A' a' P' p' b' e' : P <[b..]
+
+| conv_cast :
+  ∀ Γ i A A' B B' e e' a a',
+    Γ ⊢< Ax i > A ≡ A' : Sort i ->
+    Γ ⊢< Ax i > B ≡ B' : Sort i ->
+    Γ ⊢< prop > e ≡ e' : obseq (Ax i) (Sort i) A B ->
+    Γ ⊢< i > a ≡ a' : A ->
+    Γ ⊢< i > cast i A B e a ≡ cast i A' B' e' a' : B
+
+| conv_injpi1 :
+  ∀ Γ i j A1 A1' A2 A2' B1 B1' B2 B2' e e',
+    Γ ⊢< Ax i > A1 ≡ A1' : Sort i ->
+    Γ ,, (i, A1) ⊢< Ax j > B1 ≡ B1' : Sort j ->
+    Γ ⊢< Ax i > A2 ≡ A2' : Sort i ->
+    Γ ,, (i, A2) ⊢< Ax j > B2 ≡ B2' : Sort j ->
+    Γ ⊢< prop > e ≡ e' : obseq (Ax (Ru i j)) (Sort (Ru i j)) (Pi i j A1 B1) (Pi i j A2 B2) ->
+    Γ ⊢< prop > injpi1 i j A1 A2 B1 B2 e ≡ injpi1 i j A1' A2' B1' B2' e' : obseq (Ax i) (Sort i) A2 A1
+
+| conv_injpi2 :
+  ∀ Γ i j A1 A1' A2 A2' B1 B1' B2 B2' e e' a2 a2',
+    Γ ⊢< Ax i > A1 ≡ A1' : Sort i ->
+    Γ ,, (i, A1) ⊢< Ax j > B1 ≡ B1' : Sort j ->
+    Γ ⊢< Ax i > A2 ≡ A2' : Sort i ->
+    Γ ,, (i, A2) ⊢< Ax j > B2 ≡ B2' : Sort j ->
+    Γ ⊢< prop > e ≡ e' : obseq (Ax (Ru i j)) (Sort (Ru i j)) (Pi i j A1 B1) (Pi i j A2 B2) ->
+    Γ ⊢< i > a2 ≡ a2' : A2 ->
+    let a1 := cast i A2 A1 (injpi1 i j A1 A2 B1 B2 e) a2 in
+    Γ ⊢< prop > injpi2 i j A1 A2 B1 B2 e a2 ≡ injpi2 i j A1' A2' B1' B2' e' a2' : obseq (Ax j) (Sort j) (B1<[a1..]) (B2 <[a2..])
+
+| conv_cast_refl :
+    ∀ Γ i A B e a,
+      Γ ⊢< Ax i > A ≡ B : Sort i ->
+      Γ ⊢< prop > e : obseq (Ax i) (Sort i) A B ->
+      Γ ⊢< i > a : A ->
+      Γ ⊢< i > cast i A B e a ≡ a : B
+
+| conv_cast_pi :
+  ∀ Γ i j A1 A2 B1 B2 e f,
+    Γ ⊢< Ax i > A1 : Sort i ->
+    Γ ,, (i, A1) ⊢< Ax j > B1 : Sort j ->
+    Γ ⊢< Ax i > A2 : Sort i ->
+    Γ ,, (i, A2) ⊢< Ax j > B2 : Sort j ->
+    Γ ⊢< prop > e : obseq (Ax (Ru i j)) (Sort (Ru i j)) (Pi i j A1 B1) (Pi i j A2 B2) ->
+    Γ ⊢< Ru i j > f : Pi i j A1 B1 ->
+    let A1' := S ⋅ A1 in
+    let A2' := S ⋅ A2 in
+    let B1' := (up_ren S) ⋅ B1 in
+    let B2' := (up_ren S) ⋅ B2 in
+    let t1 := cast i A2' A1' (injpi1 i j A1' A2' B1' B2' (S ⋅ e)) (var 0) in
+    let t2 := app i j A1' B1' (S ⋅ f) t1 in
+    let t3 := cast j (B1 <[t1.: S >> var]) B2 (injpi2 i j A1' A2' B1' B2' (S ⋅ e) (var 0)) t2 in
+    let t4 := lam i j A2 B2 t3 in
+    Γ ⊢< Ru i j > cast (Ru i j) (Pi i j A1 B1) (Pi i j A2 B2) e f ≡ t4 : Pi i j A2 B2
+
+
+| conv_conv :
+    ∀ Γ l A B t t',
+      Γ ⊢< l > t ≡ t' : A ->
+      Γ ⊢< Ax l > A ≡ B : Sort l ->
+      Γ ⊢< l > t ≡ t' : B
+
+| conv_irrel :
+    ∀ Γ A t t',
+      Γ ⊢< prop > t : A ->
+      Γ ⊢< prop > t' : A ->
+      Γ ⊢< prop > t ≡ t' : A
+
+| conv_beta :
+    ∀ Γ i j A B t u,
+      Γ ⊢< Ax i > A : Sort i →
+      Γ ,, (i , A) ⊢< Ax j > B : Sort j →
+      Γ ,, (i , A) ⊢< j > t : B →
+      Γ ⊢< i > u : A →
+      Γ ⊢< j > app i j A B (lam i j A B t) u ≡ t <[ u .. ] : B <[ u .. ]
+
+| conv_eta :
+    ∀ Γ i j A B t u,
+      Γ ⊢< Ax i > A : Sort i →
+      Γ ,, (i , A) ⊢< Ax j > B : Sort j →
+      Γ ⊢< Ru i j > t : Pi i j A B →
+      Γ ⊢< Ru i j > u : Pi i j A B →
+      let t_app_x := app i j (S ⋅ A) ((up_ren S) ⋅ B) (S ⋅ t) (var 0) in
+      let u_app_x := app i j (S ⋅ A) ((up_ren S) ⋅ B) (S ⋅ u) (var 0) in
+      Γ ,, (i , A) ⊢< j > t_app_x ≡ u_app_x : B →
+      Γ ⊢< Ru i j > t ≡ u : Pi i j A B
+
+| conv_rec_zero :
+    ∀ Γ l P p_zero p_succ,
+      Γ ,, (ty 0 , Nat) ⊢< Ax l > P : Sort l ->
+      Γ ⊢< l > p_zero : P <[ zero .. ] ->
+      Γ ,, (ty 0 , Nat) ,, (l , P) ⊢< l > p_succ : P <[ (succ (var 1)) .: (shift >> (shift >> var)) ]  ->
+      Γ ⊢< l > rec l P p_zero p_succ zero ≡ p_zero : P <[ zero .. ]
+
+| conv_rec_succ :
+    ∀ Γ l P p_zero p_succ t,
+      Γ ,, (ty 0 , Nat) ⊢< Ax l > P : Sort l ->
+      Γ ⊢< l > p_zero : P <[ zero .. ] ->
+      Γ ,, (ty 0 , Nat) ,, (l , P) ⊢< l > p_succ : P <[ (succ (var 1)) .: (shift >> (shift >> var)) ]  ->
+      Γ ⊢< ty 0 > t : Nat ->
+      Γ ⊢< l > rec l P p_zero p_succ (succ t) ≡
+          p_succ <[(rec l P p_zero p_succ t) .: t ..] : P <[ (succ t) .. ]
+
+| conv_accel_accin :
+    ∀ Γ i l A R a q P p,
+    Γ ⊢< Ax i > A : Sort i ->
+    Γ ,, (i, A) ,, (i, S ⋅ A) ⊢< Ax prop > R : Sort prop ->
+    Γ ,, (i, A) ⊢< Ax l > P : Sort l ->
+    let R' := R <[var 1 .: (var 0 .: (S >> S >> var))] in
+    let P' := P <[var 1 .: (S >> S >> S >> var)] in
+    let B := Pi i l (S ⋅ A) (Pi prop l R' P') in
+    let P'' := P <[var 1.: (S >> (S >> var))] in
+    Γ ,, (i, A) ,, (Ru i l, B) ⊢< l > p : P'' ->
+    Γ ⊢< i > a : A ->
+    Γ ⊢< prop > q : acc i A R a ->
+    let Awk := (S >> S) ⋅ A in
+    let Rwk := (up_ren (up_ren (S >> S))) ⋅ R in
+    let Pwk := (up_ren (S >> S)) ⋅ P in
+    let pwk := (up_ren (up_ren (S >> S))) ⋅ p in
+    let t0 := accinv i Awk Rwk ((S >> S) ⋅ a) ((S >> S) ⋅ q) (var 1) (var 0) in
+    let t1 := accel i l Awk Rwk Pwk pwk (var 1) t0 in
+    let t2 := R<[S ⋅ a .: (var 0 .: S >> var)] in
+    let t3 := lam prop l t2 P'' t1 in
+    let t4 := Pi prop l t2 P'' in
+    let t5 := lam i l A t4 t3 in
+    Γ ⊢< l > accel i l A R P p a q ≡ p <[ t5 .: a ..] : P <[a ..]
+
+| conv_sym :
+    ∀ Γ l t u A,
+      Γ ⊢< l > t ≡ u : A ->
+      Γ ⊢< l > u ≡ t : A
+
+| conv_trans :
+    ∀ Γ l t u v A,
+      Γ ⊢< l > t ≡ u : A ->
+      Γ ⊢< l > u ≡ v : A ->
+      Γ ⊢< l > t ≡ v : A
+
+where "Γ ⊢< l > t : A" := (typing Γ l t A)
+and   "⊢ Γ" := (ctx_typing Γ)
+and   "Γ ⊢< l > t ≡ u : A" := (conversion Γ l t u A).
+
+Scheme typing_mut := Induction for typing Sort Prop
+with conversion_mut := Induction for conversion Sort Prop.
+Combined Scheme typing_conversion_mutind from typing_mut, conversion_mut.
+
+Reserved Notation "Γ ⊢s σ : Δ" (at level 50, σ, Δ at next level).
+
+Reserved Notation "Γ ⊢s σ ≡ τ : Δ" (at level 50, σ, τ, Δ at next level).
+
+Inductive WellSubst (Γ : ctx) : ctx -> (nat -> term) -> Prop :=
+  | well_sempty (σ : nat -> term) :
+    Γ ⊢s σ : ∙
+  | well_scons (σ : nat -> term) (Δ : ctx) l (A : term) :
+    Γ ⊢s (↑ >> σ) : Δ ->
+    Γ ⊢< l > σ var_zero : A <[↑ >> σ] ->
+    Γ ⊢s σ : (Δ ,, (l , A))
+where "Γ ⊢s σ : Δ" := (WellSubst Γ Δ σ).
+
+Inductive ConvSubst (Γ : ctx) : ctx -> (nat -> term) -> (nat -> term) -> Prop :=
+| conv_sempty (σ τ : nat -> term) : Γ ⊢s σ ≡ τ : ∙
+| conv_scons (σ τ : nat -> term) (Δ : ctx) l A :
+  Γ ⊢s (↑ >> σ) ≡ (↑ >> τ) : Δ ->
+  Γ ⊢< l > σ var_zero ≡ τ var_zero: A <[↑ >> σ] ->
+  Γ ⊢s σ ≡ τ : Δ ,, (l , A)
+where "Γ ⊢s σ ≡ τ : Δ" := (ConvSubst Γ Δ σ τ).
+
+Reserved Notation "⊢ Γ ≡ Δ" (at level 50, Δ at next level).
+
+Inductive ConvCtx : ctx -> ctx -> Type :=
+| conv_cempty : ⊢ ∙ ≡ ∙
+| conv_ccons Γ A Δ B l :
+  ⊢ Γ ≡ Δ ->
+  Γ ⊢< Ax l > A ≡ B : Sort l ->
+  ⊢ (Γ ,, ( l , A)) ≡ (Δ ,, (l , B))
+where "⊢ Γ ≡ Δ" := (ConvCtx Γ Δ).
