theories/SetModel/autosubst/AST.v
@@ -1,0 +1,1864 @@
+From TypedConfluence Require Import core unscoped.
+From TypedConfluence Require Import BasicAST.
+From Stdlib Require Import Setoid Morphisms Relation_Definitions.
+Module Core.
+
+Inductive term : Type :=
+  | var : nat -> term
+  | Sort : level -> term
+  | assm : aref -> term
+  | Pi : level -> level -> term -> term -> term
+  | lam : level -> level -> term -> term -> term -> term
+  | app : level -> level -> term -> term -> term -> term -> term
+  | Nat : term
+  | zero : term
+  | succ : term -> term
+  | rec : level -> term -> term -> term -> term -> term
+  | acc : level -> term -> term -> term -> term
+  | accin : level -> term -> term -> term -> term -> term
+  | accinv : level -> term -> term -> term -> term -> term -> term -> term
+  | accel :
+      level -> level -> term -> term -> term -> term -> term -> term -> term
+  | obseq : level -> term -> term -> term -> term
+  | obsrefl : level -> term -> term -> term
+  | J : level -> term -> term -> term -> term -> term -> term -> term
+  | cast : level -> term -> term -> term -> term -> term
+  | injpi1 : level -> level -> term -> term -> term -> term -> term -> term
+  | injpi2 :
+      level -> level -> term -> term -> term -> term -> term -> term -> term.
+
+Lemma congr_Sort {s0 : level} {t0 : level} (H0 : s0 = t0) : Sort s0 = Sort t0.
+Proof.
+exact (eq_trans eq_refl (ap (fun x => Sort x) H0)).
+Qed.
+
+Lemma congr_assm {s0 : aref} {t0 : aref} (H0 : s0 = t0) : assm s0 = assm t0.
+Proof.
+exact (eq_trans eq_refl (ap (fun x => assm x) H0)).
+Qed.
+
+Lemma congr_Pi {s0 : level} {s1 : level} {s2 : term} {s3 : term} {t0 : level}
+  {t1 : level} {t2 : term} {t3 : term} (H0 : s0 = t0) (H1 : s1 = t1)
+  (H2 : s2 = t2) (H3 : s3 = t3) : Pi s0 s1 s2 s3 = Pi t0 t1 t2 t3.
+Proof.
+exact (eq_trans
+         (eq_trans
+            (eq_trans (eq_trans eq_refl (ap (fun x => Pi x s1 s2 s3) H0))
+               (ap (fun x => Pi t0 x s2 s3) H1))
+            (ap (fun x => Pi t0 t1 x s3) H2))
+         (ap (fun x => Pi t0 t1 t2 x) H3)).
+Qed.
+
+Lemma congr_lam {s0 : level} {s1 : level} {s2 : term} {s3 : term} {s4 : term}
+  {t0 : level} {t1 : level} {t2 : term} {t3 : term} {t4 : term}
+  (H0 : s0 = t0) (H1 : s1 = t1) (H2 : s2 = t2) (H3 : s3 = t3) (H4 : s4 = t4)
+  : lam s0 s1 s2 s3 s4 = lam t0 t1 t2 t3 t4.
+Proof.
+exact (eq_trans
+         (eq_trans
+            (eq_trans
+               (eq_trans
+                  (eq_trans eq_refl (ap (fun x => lam x s1 s2 s3 s4) H0))
+                  (ap (fun x => lam t0 x s2 s3 s4) H1))
+               (ap (fun x => lam t0 t1 x s3 s4) H2))
+            (ap (fun x => lam t0 t1 t2 x s4) H3))
+         (ap (fun x => lam t0 t1 t2 t3 x) H4)).
+Qed.
+
+Lemma congr_app {s0 : level} {s1 : level} {s2 : term} {s3 : term} {s4 : term}
+  {s5 : term} {t0 : level} {t1 : level} {t2 : term} {t3 : term} {t4 : term}
+  {t5 : term} (H0 : s0 = t0) (H1 : s1 = t1) (H2 : s2 = t2) (H3 : s3 = t3)
+  (H4 : s4 = t4) (H5 : s5 = t5) :
+  app s0 s1 s2 s3 s4 s5 = app t0 t1 t2 t3 t4 t5.
+Proof.
+exact (eq_trans
+         (eq_trans
+            (eq_trans
+               (eq_trans
+                  (eq_trans
+                     (eq_trans eq_refl
+                        (ap (fun x => app x s1 s2 s3 s4 s5) H0))
+                     (ap (fun x => app t0 x s2 s3 s4 s5) H1))
+                  (ap (fun x => app t0 t1 x s3 s4 s5) H2))
+               (ap (fun x => app t0 t1 t2 x s4 s5) H3))
+            (ap (fun x => app t0 t1 t2 t3 x s5) H4))
+         (ap (fun x => app t0 t1 t2 t3 t4 x) H5)).
+Qed.
+
+Lemma congr_Nat : Nat = Nat.
+Proof.
+exact (eq_refl).
+Qed.
+
+Lemma congr_zero : zero = zero.
+Proof.
+exact (eq_refl).
+Qed.
+
+Lemma congr_succ {s0 : term} {t0 : term} (H0 : s0 = t0) : succ s0 = succ t0.
+Proof.
+exact (eq_trans eq_refl (ap (fun x => succ x) H0)).
+Qed.
+
+Lemma congr_rec {s0 : level} {s1 : term} {s2 : term} {s3 : term} {s4 : term}
+  {t0 : level} {t1 : term} {t2 : term} {t3 : term} {t4 : term} (H0 : s0 = t0)
+  (H1 : s1 = t1) (H2 : s2 = t2) (H3 : s3 = t3) (H4 : s4 = t4) :
+  rec s0 s1 s2 s3 s4 = rec t0 t1 t2 t3 t4.
+Proof.
+exact (eq_trans
+         (eq_trans
+            (eq_trans
+               (eq_trans
+                  (eq_trans eq_refl (ap (fun x => rec x s1 s2 s3 s4) H0))
+                  (ap (fun x => rec t0 x s2 s3 s4) H1))
+               (ap (fun x => rec t0 t1 x s3 s4) H2))
+            (ap (fun x => rec t0 t1 t2 x s4) H3))
+         (ap (fun x => rec t0 t1 t2 t3 x) H4)).
+Qed.
+
+Lemma congr_acc {s0 : level} {s1 : term} {s2 : term} {s3 : term} {t0 : level}
+  {t1 : term} {t2 : term} {t3 : term} (H0 : s0 = t0) (H1 : s1 = t1)
+  (H2 : s2 = t2) (H3 : s3 = t3) : acc s0 s1 s2 s3 = acc t0 t1 t2 t3.
+Proof.
+exact (eq_trans
+         (eq_trans
+            (eq_trans (eq_trans eq_refl (ap (fun x => acc x s1 s2 s3) H0))
+               (ap (fun x => acc t0 x s2 s3) H1))
+            (ap (fun x => acc t0 t1 x s3) H2))
+         (ap (fun x => acc t0 t1 t2 x) H3)).
+Qed.
+
+Lemma congr_accin {s0 : level} {s1 : term} {s2 : term} {s3 : term}
+  {s4 : term} {t0 : level} {t1 : term} {t2 : term} {t3 : term} {t4 : term}
+  (H0 : s0 = t0) (H1 : s1 = t1) (H2 : s2 = t2) (H3 : s3 = t3) (H4 : s4 = t4)
+  : accin s0 s1 s2 s3 s4 = accin t0 t1 t2 t3 t4.
+Proof.
+exact (eq_trans
+         (eq_trans
+            (eq_trans
+               (eq_trans
+                  (eq_trans eq_refl (ap (fun x => accin x s1 s2 s3 s4) H0))
+                  (ap (fun x => accin t0 x s2 s3 s4) H1))
+               (ap (fun x => accin t0 t1 x s3 s4) H2))
+            (ap (fun x => accin t0 t1 t2 x s4) H3))
+         (ap (fun x => accin t0 t1 t2 t3 x) H4)).
+Qed.
+
+Lemma congr_accinv {s0 : level} {s1 : term} {s2 : term} {s3 : term}
+  {s4 : term} {s5 : term} {s6 : term} {t0 : level} {t1 : term} {t2 : term}
+  {t3 : term} {t4 : term} {t5 : term} {t6 : term} (H0 : s0 = t0)
+  (H1 : s1 = t1) (H2 : s2 = t2) (H3 : s3 = t3) (H4 : s4 = t4) (H5 : s5 = t5)
+  (H6 : s6 = t6) : accinv s0 s1 s2 s3 s4 s5 s6 = accinv t0 t1 t2 t3 t4 t5 t6.
+Proof.
+exact (eq_trans
+         (eq_trans
+            (eq_trans
+               (eq_trans
+                  (eq_trans
+                     (eq_trans
+                        (eq_trans eq_refl
+                           (ap (fun x => accinv x s1 s2 s3 s4 s5 s6) H0))
+                        (ap (fun x => accinv t0 x s2 s3 s4 s5 s6) H1))
+                     (ap (fun x => accinv t0 t1 x s3 s4 s5 s6) H2))
+                  (ap (fun x => accinv t0 t1 t2 x s4 s5 s6) H3))
+               (ap (fun x => accinv t0 t1 t2 t3 x s5 s6) H4))
+            (ap (fun x => accinv t0 t1 t2 t3 t4 x s6) H5))
+         (ap (fun x => accinv t0 t1 t2 t3 t4 t5 x) H6)).
+Qed.
+
+Lemma congr_accel {s0 : level} {s1 : level} {s2 : term} {s3 : term}
+  {s4 : term} {s5 : term} {s6 : term} {s7 : term} {t0 : level} {t1 : level}
+  {t2 : term} {t3 : term} {t4 : term} {t5 : term} {t6 : term} {t7 : term}
+  (H0 : s0 = t0) (H1 : s1 = t1) (H2 : s2 = t2) (H3 : s3 = t3) (H4 : s4 = t4)
+  (H5 : s5 = t5) (H6 : s6 = t6) (H7 : s7 = t7) :
+  accel s0 s1 s2 s3 s4 s5 s6 s7 = accel t0 t1 t2 t3 t4 t5 t6 t7.
+Proof.
+exact (eq_trans
+         (eq_trans
+            (eq_trans
+               (eq_trans
+                  (eq_trans
+                     (eq_trans
+                        (eq_trans
+                           (eq_trans eq_refl
+                              (ap (fun x => accel x s1 s2 s3 s4 s5 s6 s7) H0))
+                           (ap (fun x => accel t0 x s2 s3 s4 s5 s6 s7) H1))
+                        (ap (fun x => accel t0 t1 x s3 s4 s5 s6 s7) H2))
+                     (ap (fun x => accel t0 t1 t2 x s4 s5 s6 s7) H3))
+                  (ap (fun x => accel t0 t1 t2 t3 x s5 s6 s7) H4))
+               (ap (fun x => accel t0 t1 t2 t3 t4 x s6 s7) H5))
+            (ap (fun x => accel t0 t1 t2 t3 t4 t5 x s7) H6))
+         (ap (fun x => accel t0 t1 t2 t3 t4 t5 t6 x) H7)).
+Qed.
+
+Lemma congr_obseq {s0 : level} {s1 : term} {s2 : term} {s3 : term}
+  {t0 : level} {t1 : term} {t2 : term} {t3 : term} (H0 : s0 = t0)
+  (H1 : s1 = t1) (H2 : s2 = t2) (H3 : s3 = t3) :
+  obseq s0 s1 s2 s3 = obseq t0 t1 t2 t3.
+Proof.
+exact (eq_trans
+         (eq_trans
+            (eq_trans (eq_trans eq_refl (ap (fun x => obseq x s1 s2 s3) H0))
+               (ap (fun x => obseq t0 x s2 s3) H1))
+            (ap (fun x => obseq t0 t1 x s3) H2))
+         (ap (fun x => obseq t0 t1 t2 x) H3)).
+Qed.
+
+Lemma congr_obsrefl {s0 : level} {s1 : term} {s2 : term} {t0 : level}
+  {t1 : term} {t2 : term} (H0 : s0 = t0) (H1 : s1 = t1) (H2 : s2 = t2) :
+  obsrefl s0 s1 s2 = obsrefl t0 t1 t2.
+Proof.
+exact (eq_trans
+         (eq_trans (eq_trans eq_refl (ap (fun x => obsrefl x s1 s2) H0))
+            (ap (fun x => obsrefl t0 x s2) H1))
+         (ap (fun x => obsrefl t0 t1 x) H2)).
+Qed.
+
+Lemma congr_J {s0 : level} {s1 : term} {s2 : term} {s3 : term} {s4 : term}
+  {s5 : term} {s6 : term} {t0 : level} {t1 : term} {t2 : term} {t3 : term}
+  {t4 : term} {t5 : term} {t6 : term} (H0 : s0 = t0) (H1 : s1 = t1)
+  (H2 : s2 = t2) (H3 : s3 = t3) (H4 : s4 = t4) (H5 : s5 = t5) (H6 : s6 = t6)
+  : J s0 s1 s2 s3 s4 s5 s6 = J t0 t1 t2 t3 t4 t5 t6.
+Proof.
+exact (eq_trans
+         (eq_trans
+            (eq_trans
+               (eq_trans
+                  (eq_trans
+                     (eq_trans
+                        (eq_trans eq_refl
+                           (ap (fun x => J x s1 s2 s3 s4 s5 s6) H0))
+                        (ap (fun x => J t0 x s2 s3 s4 s5 s6) H1))
+                     (ap (fun x => J t0 t1 x s3 s4 s5 s6) H2))
+                  (ap (fun x => J t0 t1 t2 x s4 s5 s6) H3))
+               (ap (fun x => J t0 t1 t2 t3 x s5 s6) H4))
+            (ap (fun x => J t0 t1 t2 t3 t4 x s6) H5))
+         (ap (fun x => J t0 t1 t2 t3 t4 t5 x) H6)).
+Qed.
+
+Lemma congr_cast {s0 : level} {s1 : term} {s2 : term} {s3 : term} {s4 : term}
+  {t0 : level} {t1 : term} {t2 : term} {t3 : term} {t4 : term} (H0 : s0 = t0)
+  (H1 : s1 = t1) (H2 : s2 = t2) (H3 : s3 = t3) (H4 : s4 = t4) :
+  cast s0 s1 s2 s3 s4 = cast t0 t1 t2 t3 t4.
+Proof.
+exact (eq_trans
+         (eq_trans
+            (eq_trans
+               (eq_trans
+                  (eq_trans eq_refl (ap (fun x => cast x s1 s2 s3 s4) H0))
+                  (ap (fun x => cast t0 x s2 s3 s4) H1))
+               (ap (fun x => cast t0 t1 x s3 s4) H2))
+            (ap (fun x => cast t0 t1 t2 x s4) H3))
+         (ap (fun x => cast t0 t1 t2 t3 x) H4)).
+Qed.
+
+Lemma congr_injpi1 {s0 : level} {s1 : level} {s2 : term} {s3 : term}
+  {s4 : term} {s5 : term} {s6 : term} {t0 : level} {t1 : level} {t2 : term}
+  {t3 : term} {t4 : term} {t5 : term} {t6 : term} (H0 : s0 = t0)
+  (H1 : s1 = t1) (H2 : s2 = t2) (H3 : s3 = t3) (H4 : s4 = t4) (H5 : s5 = t5)
+  (H6 : s6 = t6) : injpi1 s0 s1 s2 s3 s4 s5 s6 = injpi1 t0 t1 t2 t3 t4 t5 t6.
+Proof.
+exact (eq_trans
+         (eq_trans
+            (eq_trans
+               (eq_trans
+                  (eq_trans
+                     (eq_trans
+                        (eq_trans eq_refl
+                           (ap (fun x => injpi1 x s1 s2 s3 s4 s5 s6) H0))
+                        (ap (fun x => injpi1 t0 x s2 s3 s4 s5 s6) H1))
+                     (ap (fun x => injpi1 t0 t1 x s3 s4 s5 s6) H2))
+                  (ap (fun x => injpi1 t0 t1 t2 x s4 s5 s6) H3))
+               (ap (fun x => injpi1 t0 t1 t2 t3 x s5 s6) H4))
+            (ap (fun x => injpi1 t0 t1 t2 t3 t4 x s6) H5))
+         (ap (fun x => injpi1 t0 t1 t2 t3 t4 t5 x) H6)).
+Qed.
+
+Lemma congr_injpi2 {s0 : level} {s1 : level} {s2 : term} {s3 : term}
+  {s4 : term} {s5 : term} {s6 : term} {s7 : term} {t0 : level} {t1 : level}
+  {t2 : term} {t3 : term} {t4 : term} {t5 : term} {t6 : term} {t7 : term}
+  (H0 : s0 = t0) (H1 : s1 = t1) (H2 : s2 = t2) (H3 : s3 = t3) (H4 : s4 = t4)
+  (H5 : s5 = t5) (H6 : s6 = t6) (H7 : s7 = t7) :
+  injpi2 s0 s1 s2 s3 s4 s5 s6 s7 = injpi2 t0 t1 t2 t3 t4 t5 t6 t7.
+Proof.
+exact (eq_trans
+         (eq_trans
+            (eq_trans
+               (eq_trans
+                  (eq_trans
+                     (eq_trans
+                        (eq_trans
+                           (eq_trans eq_refl
+                              (ap (fun x => injpi2 x s1 s2 s3 s4 s5 s6 s7) H0))
+                           (ap (fun x => injpi2 t0 x s2 s3 s4 s5 s6 s7) H1))
+                        (ap (fun x => injpi2 t0 t1 x s3 s4 s5 s6 s7) H2))
+                     (ap (fun x => injpi2 t0 t1 t2 x s4 s5 s6 s7) H3))
+                  (ap (fun x => injpi2 t0 t1 t2 t3 x s5 s6 s7) H4))
+               (ap (fun x => injpi2 t0 t1 t2 t3 t4 x s6 s7) H5))
+            (ap (fun x => injpi2 t0 t1 t2 t3 t4 t5 x s7) H6))
+         (ap (fun x => injpi2 t0 t1 t2 t3 t4 t5 t6 x) H7)).
+Qed.
+
+Lemma upRen_term_term (xi : nat -> nat) : nat -> nat.
+Proof.
+exact (up_ren xi).
+Defined.
+
+Fixpoint ren_term (xi_term : nat -> nat) (s : term) {struct s} : term :=
+  match s with
+  | var s0 => var (xi_term s0)
+  | Sort s0 => Sort s0
+  | assm s0 => assm s0
+  | Pi s0 s1 s2 s3 =>
+      Pi s0 s1 (ren_term xi_term s2) (ren_term (upRen_term_term xi_term) s3)
+  | lam s0 s1 s2 s3 s4 =>
+      lam s0 s1 (ren_term xi_term s2) (ren_term (upRen_term_term xi_term) s3)
+        (ren_term (upRen_term_term xi_term) s4)
+  | app s0 s1 s2 s3 s4 s5 =>
+      app s0 s1 (ren_term xi_term s2) (ren_term (upRen_term_term xi_term) s3)
+        (ren_term xi_term s4) (ren_term xi_term s5)
+  | Nat => Nat
+  | zero => zero
+  | succ s0 => succ (ren_term xi_term s0)
+  | rec s0 s1 s2 s3 s4 =>
+      rec s0 (ren_term (upRen_term_term xi_term) s1) (ren_term xi_term s2)
+        (ren_term (upRen_term_term (upRen_term_term xi_term)) s3)
+        (ren_term xi_term s4)
+  | acc s0 s1 s2 s3 =>
+      acc s0 (ren_term xi_term s1)
+        (ren_term (upRen_term_term (upRen_term_term xi_term)) s2)
+        (ren_term xi_term s3)
+  | accin s0 s1 s2 s3 s4 =>
+      accin s0 (ren_term xi_term s1)
+        (ren_term (upRen_term_term (upRen_term_term xi_term)) s2)
+        (ren_term xi_term s3) (ren_term xi_term s4)
+  | accinv s0 s1 s2 s3 s4 s5 s6 =>
+      accinv s0 (ren_term xi_term s1)
+        (ren_term (upRen_term_term (upRen_term_term xi_term)) s2)
+        (ren_term xi_term s3) (ren_term xi_term s4) (ren_term xi_term s5)
+        (ren_term xi_term s6)
+  | accel s0 s1 s2 s3 s4 s5 s6 s7 =>
+      accel s0 s1 (ren_term xi_term s2)
+        (ren_term (upRen_term_term (upRen_term_term xi_term)) s3)
+        (ren_term (upRen_term_term xi_term) s4)
+        (ren_term (upRen_term_term (upRen_term_term xi_term)) s5)
+        (ren_term xi_term s6) (ren_term xi_term s7)
+  | obseq s0 s1 s2 s3 =>
+      obseq s0 (ren_term xi_term s1) (ren_term xi_term s2)
+        (ren_term xi_term s3)
+  | obsrefl s0 s1 s2 =>
+      obsrefl s0 (ren_term xi_term s1) (ren_term xi_term s2)
+  | J s0 s1 s2 s3 s4 s5 s6 =>
+      J s0 (ren_term xi_term s1) (ren_term xi_term s2)
+        (ren_term (upRen_term_term xi_term) s3) (ren_term xi_term s4)
+        (ren_term xi_term s5) (ren_term xi_term s6)
+  | cast s0 s1 s2 s3 s4 =>
+      cast s0 (ren_term xi_term s1) (ren_term xi_term s2)
+        (ren_term xi_term s3) (ren_term xi_term s4)
+  | injpi1 s0 s1 s2 s3 s4 s5 s6 =>
+      injpi1 s0 s1 (ren_term xi_term s2) (ren_term xi_term s3)
+        (ren_term (upRen_term_term xi_term) s4)
+        (ren_term (upRen_term_term xi_term) s5) (ren_term xi_term s6)
+  | injpi2 s0 s1 s2 s3 s4 s5 s6 s7 =>
+      injpi2 s0 s1 (ren_term xi_term s2) (ren_term xi_term s3)
+        (ren_term (upRen_term_term xi_term) s4)
+        (ren_term (upRen_term_term xi_term) s5) (ren_term xi_term s6)
+        (ren_term xi_term s7)
+  end.
+
+Lemma up_term_term (sigma : nat -> term) : nat -> term.
+Proof.
+exact (scons (var var_zero) (funcomp (ren_term shift) sigma)).
+Defined.
+
+Fixpoint subst_term (sigma_term : nat -> term) (s : term) {struct s} : 
+term :=
+  match s with
+  | var s0 => sigma_term s0
+  | Sort s0 => Sort s0
+  | assm s0 => assm s0
+  | Pi s0 s1 s2 s3 =>
+      Pi s0 s1 (subst_term sigma_term s2)
+        (subst_term (up_term_term sigma_term) s3)
+  | lam s0 s1 s2 s3 s4 =>
+      lam s0 s1 (subst_term sigma_term s2)
+        (subst_term (up_term_term sigma_term) s3)
+        (subst_term (up_term_term sigma_term) s4)
+  | app s0 s1 s2 s3 s4 s5 =>
+      app s0 s1 (subst_term sigma_term s2)
+        (subst_term (up_term_term sigma_term) s3) (subst_term sigma_term s4)
+        (subst_term sigma_term s5)
+  | Nat => Nat
+  | zero => zero
+  | succ s0 => succ (subst_term sigma_term s0)
+  | rec s0 s1 s2 s3 s4 =>
+      rec s0 (subst_term (up_term_term sigma_term) s1)
+        (subst_term sigma_term s2)
+        (subst_term (up_term_term (up_term_term sigma_term)) s3)
+        (subst_term sigma_term s4)
+  | acc s0 s1 s2 s3 =>
+      acc s0 (subst_term sigma_term s1)
+        (subst_term (up_term_term (up_term_term sigma_term)) s2)
+        (subst_term sigma_term s3)
+  | accin s0 s1 s2 s3 s4 =>
+      accin s0 (subst_term sigma_term s1)
+        (subst_term (up_term_term (up_term_term sigma_term)) s2)
+        (subst_term sigma_term s3) (subst_term sigma_term s4)
+  | accinv s0 s1 s2 s3 s4 s5 s6 =>
+      accinv s0 (subst_term sigma_term s1)
+        (subst_term (up_term_term (up_term_term sigma_term)) s2)
+        (subst_term sigma_term s3) (subst_term sigma_term s4)
+        (subst_term sigma_term s5) (subst_term sigma_term s6)
+  | accel s0 s1 s2 s3 s4 s5 s6 s7 =>
+      accel s0 s1 (subst_term sigma_term s2)
+        (subst_term (up_term_term (up_term_term sigma_term)) s3)
+        (subst_term (up_term_term sigma_term) s4)
+        (subst_term (up_term_term (up_term_term sigma_term)) s5)
+        (subst_term sigma_term s6) (subst_term sigma_term s7)
+  | obseq s0 s1 s2 s3 =>
+      obseq s0 (subst_term sigma_term s1) (subst_term sigma_term s2)
+        (subst_term sigma_term s3)
+  | obsrefl s0 s1 s2 =>
+      obsrefl s0 (subst_term sigma_term s1) (subst_term sigma_term s2)
+  | J s0 s1 s2 s3 s4 s5 s6 =>
+      J s0 (subst_term sigma_term s1) (subst_term sigma_term s2)
+        (subst_term (up_term_term sigma_term) s3) (subst_term sigma_term s4)
+        (subst_term sigma_term s5) (subst_term sigma_term s6)
+  | cast s0 s1 s2 s3 s4 =>
+      cast s0 (subst_term sigma_term s1) (subst_term sigma_term s2)
+        (subst_term sigma_term s3) (subst_term sigma_term s4)
+  | injpi1 s0 s1 s2 s3 s4 s5 s6 =>
+      injpi1 s0 s1 (subst_term sigma_term s2) (subst_term sigma_term s3)
+        (subst_term (up_term_term sigma_term) s4)
+        (subst_term (up_term_term sigma_term) s5) (subst_term sigma_term s6)
+  | injpi2 s0 s1 s2 s3 s4 s5 s6 s7 =>
+      injpi2 s0 s1 (subst_term sigma_term s2) (subst_term sigma_term s3)
+        (subst_term (up_term_term sigma_term) s4)
+        (subst_term (up_term_term sigma_term) s5) (subst_term sigma_term s6)
+        (subst_term sigma_term s7)
+  end.
+
+Lemma upId_term_term (sigma : nat -> term) (Eq : forall x, sigma x = var x) :
+  forall x, up_term_term sigma x = var x.
+Proof.
+exact (fun n =>
+       match n with
+       | S n' => ap (ren_term shift) (Eq n')
+       | O => eq_refl
+       end).
+Qed.
+
+Fixpoint idSubst_term (sigma_term : nat -> term)
+(Eq_term : forall x, sigma_term x = var x) (s : term) {struct s} :
+subst_term sigma_term s = s :=
+  match s with
+  | var s0 => Eq_term s0
+  | Sort s0 => congr_Sort (eq_refl s0)
+  | assm s0 => congr_assm (eq_refl s0)
+  | Pi s0 s1 s2 s3 =>
+      congr_Pi (eq_refl s0) (eq_refl s1) (idSubst_term sigma_term Eq_term s2)
+        (idSubst_term (up_term_term sigma_term) (upId_term_term _ Eq_term) s3)
+  | lam s0 s1 s2 s3 s4 =>
+      congr_lam (eq_refl s0) (eq_refl s1)
+        (idSubst_term sigma_term Eq_term s2)
+        (idSubst_term (up_term_term sigma_term) (upId_term_term _ Eq_term) s3)
+        (idSubst_term (up_term_term sigma_term) (upId_term_term _ Eq_term) s4)
+  | app s0 s1 s2 s3 s4 s5 =>
+      congr_app (eq_refl s0) (eq_refl s1)
+        (idSubst_term sigma_term Eq_term s2)
+        (idSubst_term (up_term_term sigma_term) (upId_term_term _ Eq_term) s3)
+        (idSubst_term sigma_term Eq_term s4)
+        (idSubst_term sigma_term Eq_term s5)
+  | Nat => congr_Nat
+  | zero => congr_zero
+  | succ s0 => congr_succ (idSubst_term sigma_term Eq_term s0)
+  | rec s0 s1 s2 s3 s4 =>
+      congr_rec (eq_refl s0)
+        (idSubst_term (up_term_term sigma_term) (upId_term_term _ Eq_term) s1)
+        (idSubst_term sigma_term Eq_term s2)
+        (idSubst_term (up_term_term (up_term_term sigma_term))
+           (upId_term_term _ (upId_term_term _ Eq_term)) s3)
+        (idSubst_term sigma_term Eq_term s4)
+  | acc s0 s1 s2 s3 =>
+      congr_acc (eq_refl s0) (idSubst_term sigma_term Eq_term s1)
+        (idSubst_term (up_term_term (up_term_term sigma_term))
+           (upId_term_term _ (upId_term_term _ Eq_term)) s2)
+        (idSubst_term sigma_term Eq_term s3)
+  | accin s0 s1 s2 s3 s4 =>
+      congr_accin (eq_refl s0) (idSubst_term sigma_term Eq_term s1)
+        (idSubst_term (up_term_term (up_term_term sigma_term))
+           (upId_term_term _ (upId_term_term _ Eq_term)) s2)
+        (idSubst_term sigma_term Eq_term s3)
+        (idSubst_term sigma_term Eq_term s4)
+  | accinv s0 s1 s2 s3 s4 s5 s6 =>
+      congr_accinv (eq_refl s0) (idSubst_term sigma_term Eq_term s1)
+        (idSubst_term (up_term_term (up_term_term sigma_term))
+           (upId_term_term _ (upId_term_term _ Eq_term)) s2)
+        (idSubst_term sigma_term Eq_term s3)
+        (idSubst_term sigma_term Eq_term s4)
+        (idSubst_term sigma_term Eq_term s5)
+        (idSubst_term sigma_term Eq_term s6)
+  | accel s0 s1 s2 s3 s4 s5 s6 s7 =>
+      congr_accel (eq_refl s0) (eq_refl s1)
+        (idSubst_term sigma_term Eq_term s2)
+        (idSubst_term (up_term_term (up_term_term sigma_term))
+           (upId_term_term _ (upId_term_term _ Eq_term)) s3)
+        (idSubst_term (up_term_term sigma_term) (upId_term_term _ Eq_term) s4)
+        (idSubst_term (up_term_term (up_term_term sigma_term))
+           (upId_term_term _ (upId_term_term _ Eq_term)) s5)
+        (idSubst_term sigma_term Eq_term s6)
+        (idSubst_term sigma_term Eq_term s7)
+  | obseq s0 s1 s2 s3 =>
+      congr_obseq (eq_refl s0) (idSubst_term sigma_term Eq_term s1)
+        (idSubst_term sigma_term Eq_term s2)
+        (idSubst_term sigma_term Eq_term s3)
+  | obsrefl s0 s1 s2 =>
+      congr_obsrefl (eq_refl s0) (idSubst_term sigma_term Eq_term s1)
+        (idSubst_term sigma_term Eq_term s2)
+  | J s0 s1 s2 s3 s4 s5 s6 =>
+      congr_J (eq_refl s0) (idSubst_term sigma_term Eq_term s1)
+        (idSubst_term sigma_term Eq_term s2)
+        (idSubst_term (up_term_term sigma_term) (upId_term_term _ Eq_term) s3)
+        (idSubst_term sigma_term Eq_term s4)
+        (idSubst_term sigma_term Eq_term s5)
+        (idSubst_term sigma_term Eq_term s6)
+  | cast s0 s1 s2 s3 s4 =>
+      congr_cast (eq_refl s0) (idSubst_term sigma_term Eq_term s1)
+        (idSubst_term sigma_term Eq_term s2)
+        (idSubst_term sigma_term Eq_term s3)
+        (idSubst_term sigma_term Eq_term s4)
+  | injpi1 s0 s1 s2 s3 s4 s5 s6 =>
+      congr_injpi1 (eq_refl s0) (eq_refl s1)
+        (idSubst_term sigma_term Eq_term s2)
+        (idSubst_term sigma_term Eq_term s3)
+        (idSubst_term (up_term_term sigma_term) (upId_term_term _ Eq_term) s4)
+        (idSubst_term (up_term_term sigma_term) (upId_term_term _ Eq_term) s5)
+        (idSubst_term sigma_term Eq_term s6)
+  | injpi2 s0 s1 s2 s3 s4 s5 s6 s7 =>
+      congr_injpi2 (eq_refl s0) (eq_refl s1)
+        (idSubst_term sigma_term Eq_term s2)
+        (idSubst_term sigma_term Eq_term s3)
+        (idSubst_term (up_term_term sigma_term) (upId_term_term _ Eq_term) s4)
+        (idSubst_term (up_term_term sigma_term) (upId_term_term _ Eq_term) s5)
+        (idSubst_term sigma_term Eq_term s6)
+        (idSubst_term sigma_term Eq_term s7)
+  end.
+
+Lemma upExtRen_term_term (xi : nat -> nat) (zeta : nat -> nat)
+  (Eq : forall x, xi x = zeta x) :
+  forall x, upRen_term_term xi x = upRen_term_term zeta x.
+Proof.
+exact (fun n => match n with
+                | S n' => ap shift (Eq n')
+                | O => eq_refl
+                end).
+Qed.
+
+Fixpoint extRen_term (xi_term : nat -> nat) (zeta_term : nat -> nat)
+(Eq_term : forall x, xi_term x = zeta_term x) (s : term) {struct s} :
+ren_term xi_term s = ren_term zeta_term s :=
+  match s with
+  | var s0 => ap (var) (Eq_term s0)
+  | Sort s0 => congr_Sort (eq_refl s0)
+  | assm s0 => congr_assm (eq_refl s0)
+  | Pi s0 s1 s2 s3 =>
+      congr_Pi (eq_refl s0) (eq_refl s1)
+        (extRen_term xi_term zeta_term Eq_term s2)
+        (extRen_term (upRen_term_term xi_term) (upRen_term_term zeta_term)
+           (upExtRen_term_term _ _ Eq_term) s3)
+  | lam s0 s1 s2 s3 s4 =>
+      congr_lam (eq_refl s0) (eq_refl s1)
+        (extRen_term xi_term zeta_term Eq_term s2)
+        (extRen_term (upRen_term_term xi_term) (upRen_term_term zeta_term)
+           (upExtRen_term_term _ _ Eq_term) s3)
+        (extRen_term (upRen_term_term xi_term) (upRen_term_term zeta_term)
+           (upExtRen_term_term _ _ Eq_term) s4)
+  | app s0 s1 s2 s3 s4 s5 =>
+      congr_app (eq_refl s0) (eq_refl s1)
+        (extRen_term xi_term zeta_term Eq_term s2)
+        (extRen_term (upRen_term_term xi_term) (upRen_term_term zeta_term)
+           (upExtRen_term_term _ _ Eq_term) s3)
+        (extRen_term xi_term zeta_term Eq_term s4)
+        (extRen_term xi_term zeta_term Eq_term s5)
+  | Nat => congr_Nat
+  | zero => congr_zero
+  | succ s0 => congr_succ (extRen_term xi_term zeta_term Eq_term s0)
+  | rec s0 s1 s2 s3 s4 =>
+      congr_rec (eq_refl s0)
+        (extRen_term (upRen_term_term xi_term) (upRen_term_term zeta_term)
+           (upExtRen_term_term _ _ Eq_term) s1)
+        (extRen_term xi_term zeta_term Eq_term s2)
+        (extRen_term (upRen_term_term (upRen_term_term xi_term))
+           (upRen_term_term (upRen_term_term zeta_term))
+           (upExtRen_term_term _ _ (upExtRen_term_term _ _ Eq_term)) s3)
+        (extRen_term xi_term zeta_term Eq_term s4)
+  | acc s0 s1 s2 s3 =>
+      congr_acc (eq_refl s0) (extRen_term xi_term zeta_term Eq_term s1)
+        (extRen_term (upRen_term_term (upRen_term_term xi_term))
+           (upRen_term_term (upRen_term_term zeta_term))
+           (upExtRen_term_term _ _ (upExtRen_term_term _ _ Eq_term)) s2)
+        (extRen_term xi_term zeta_term Eq_term s3)
+  | accin s0 s1 s2 s3 s4 =>
+      congr_accin (eq_refl s0) (extRen_term xi_term zeta_term Eq_term s1)
+        (extRen_term (upRen_term_term (upRen_term_term xi_term))
+           (upRen_term_term (upRen_term_term zeta_term))
+           (upExtRen_term_term _ _ (upExtRen_term_term _ _ Eq_term)) s2)
+        (extRen_term xi_term zeta_term Eq_term s3)
+        (extRen_term xi_term zeta_term Eq_term s4)
+  | accinv s0 s1 s2 s3 s4 s5 s6 =>
+      congr_accinv (eq_refl s0) (extRen_term xi_term zeta_term Eq_term s1)
+        (extRen_term (upRen_term_term (upRen_term_term xi_term))
+           (upRen_term_term (upRen_term_term zeta_term))
+           (upExtRen_term_term _ _ (upExtRen_term_term _ _ Eq_term)) s2)
+        (extRen_term xi_term zeta_term Eq_term s3)
+        (extRen_term xi_term zeta_term Eq_term s4)
+        (extRen_term xi_term zeta_term Eq_term s5)
+        (extRen_term xi_term zeta_term Eq_term s6)
+  | accel s0 s1 s2 s3 s4 s5 s6 s7 =>
+      congr_accel (eq_refl s0) (eq_refl s1)
+        (extRen_term xi_term zeta_term Eq_term s2)
+        (extRen_term (upRen_term_term (upRen_term_term xi_term))
+           (upRen_term_term (upRen_term_term zeta_term))
+           (upExtRen_term_term _ _ (upExtRen_term_term _ _ Eq_term)) s3)
+        (extRen_term (upRen_term_term xi_term) (upRen_term_term zeta_term)
+           (upExtRen_term_term _ _ Eq_term) s4)
+        (extRen_term (upRen_term_term (upRen_term_term xi_term))
+           (upRen_term_term (upRen_term_term zeta_term))
+           (upExtRen_term_term _ _ (upExtRen_term_term _ _ Eq_term)) s5)
+        (extRen_term xi_term zeta_term Eq_term s6)
+        (extRen_term xi_term zeta_term Eq_term s7)
+  | obseq s0 s1 s2 s3 =>
+      congr_obseq (eq_refl s0) (extRen_term xi_term zeta_term Eq_term s1)
+        (extRen_term xi_term zeta_term Eq_term s2)
+        (extRen_term xi_term zeta_term Eq_term s3)
+  | obsrefl s0 s1 s2 =>
+      congr_obsrefl (eq_refl s0) (extRen_term xi_term zeta_term Eq_term s1)
+        (extRen_term xi_term zeta_term Eq_term s2)
+  | J s0 s1 s2 s3 s4 s5 s6 =>
+      congr_J (eq_refl s0) (extRen_term xi_term zeta_term Eq_term s1)
+        (extRen_term xi_term zeta_term Eq_term s2)
+        (extRen_term (upRen_term_term xi_term) (upRen_term_term zeta_term)
+           (upExtRen_term_term _ _ Eq_term) s3)
+        (extRen_term xi_term zeta_term Eq_term s4)
+        (extRen_term xi_term zeta_term Eq_term s5)
+        (extRen_term xi_term zeta_term Eq_term s6)
+  | cast s0 s1 s2 s3 s4 =>
+      congr_cast (eq_refl s0) (extRen_term xi_term zeta_term Eq_term s1)
+        (extRen_term xi_term zeta_term Eq_term s2)
+        (extRen_term xi_term zeta_term Eq_term s3)
+        (extRen_term xi_term zeta_term Eq_term s4)
+  | injpi1 s0 s1 s2 s3 s4 s5 s6 =>
+      congr_injpi1 (eq_refl s0) (eq_refl s1)
+        (extRen_term xi_term zeta_term Eq_term s2)
+        (extRen_term xi_term zeta_term Eq_term s3)
+        (extRen_term (upRen_term_term xi_term) (upRen_term_term zeta_term)
+           (upExtRen_term_term _ _ Eq_term) s4)
+        (extRen_term (upRen_term_term xi_term) (upRen_term_term zeta_term)
+           (upExtRen_term_term _ _ Eq_term) s5)
+        (extRen_term xi_term zeta_term Eq_term s6)
+  | injpi2 s0 s1 s2 s3 s4 s5 s6 s7 =>
+      congr_injpi2 (eq_refl s0) (eq_refl s1)
+        (extRen_term xi_term zeta_term Eq_term s2)
+        (extRen_term xi_term zeta_term Eq_term s3)
+        (extRen_term (upRen_term_term xi_term) (upRen_term_term zeta_term)
+           (upExtRen_term_term _ _ Eq_term) s4)
+        (extRen_term (upRen_term_term xi_term) (upRen_term_term zeta_term)
+           (upExtRen_term_term _ _ Eq_term) s5)
+        (extRen_term xi_term zeta_term Eq_term s6)
+        (extRen_term xi_term zeta_term Eq_term s7)
+  end.
+
+Lemma upExt_term_term (sigma : nat -> term) (tau : nat -> term)
+  (Eq : forall x, sigma x = tau x) :
+  forall x, up_term_term sigma x = up_term_term tau x.
+Proof.
+exact (fun n =>
+       match n with
+       | S n' => ap (ren_term shift) (Eq n')
+       | O => eq_refl
+       end).
+Qed.
+
+Fixpoint ext_term (sigma_term : nat -> term) (tau_term : nat -> term)
+(Eq_term : forall x, sigma_term x = tau_term x) (s : term) {struct s} :
+subst_term sigma_term s = subst_term tau_term s :=
+  match s with
+  | var s0 => Eq_term s0
+  | Sort s0 => congr_Sort (eq_refl s0)
+  | assm s0 => congr_assm (eq_refl s0)
+  | Pi s0 s1 s2 s3 =>
+      congr_Pi (eq_refl s0) (eq_refl s1)
+        (ext_term sigma_term tau_term Eq_term s2)
+        (ext_term (up_term_term sigma_term) (up_term_term tau_term)
+           (upExt_term_term _ _ Eq_term) s3)
+  | lam s0 s1 s2 s3 s4 =>
+      congr_lam (eq_refl s0) (eq_refl s1)
+        (ext_term sigma_term tau_term Eq_term s2)
+        (ext_term (up_term_term sigma_term) (up_term_term tau_term)
+           (upExt_term_term _ _ Eq_term) s3)
+        (ext_term (up_term_term sigma_term) (up_term_term tau_term)
+           (upExt_term_term _ _ Eq_term) s4)
+  | app s0 s1 s2 s3 s4 s5 =>
+      congr_app (eq_refl s0) (eq_refl s1)
+        (ext_term sigma_term tau_term Eq_term s2)
+        (ext_term (up_term_term sigma_term) (up_term_term tau_term)
+           (upExt_term_term _ _ Eq_term) s3)
+        (ext_term sigma_term tau_term Eq_term s4)
+        (ext_term sigma_term tau_term Eq_term s5)
+  | Nat => congr_Nat
+  | zero => congr_zero
+  | succ s0 => congr_succ (ext_term sigma_term tau_term Eq_term s0)
+  | rec s0 s1 s2 s3 s4 =>
+      congr_rec (eq_refl s0)
+        (ext_term (up_term_term sigma_term) (up_term_term tau_term)
+           (upExt_term_term _ _ Eq_term) s1)
+        (ext_term sigma_term tau_term Eq_term s2)
+        (ext_term (up_term_term (up_term_term sigma_term))
+           (up_term_term (up_term_term tau_term))
+           (upExt_term_term _ _ (upExt_term_term _ _ Eq_term)) s3)
+        (ext_term sigma_term tau_term Eq_term s4)
+  | acc s0 s1 s2 s3 =>
+      congr_acc (eq_refl s0) (ext_term sigma_term tau_term Eq_term s1)
+        (ext_term (up_term_term (up_term_term sigma_term))
+           (up_term_term (up_term_term tau_term))
+           (upExt_term_term _ _ (upExt_term_term _ _ Eq_term)) s2)
+        (ext_term sigma_term tau_term Eq_term s3)
+  | accin s0 s1 s2 s3 s4 =>
+      congr_accin (eq_refl s0) (ext_term sigma_term tau_term Eq_term s1)
+        (ext_term (up_term_term (up_term_term sigma_term))
+           (up_term_term (up_term_term tau_term))
+           (upExt_term_term _ _ (upExt_term_term _ _ Eq_term)) s2)
+        (ext_term sigma_term tau_term Eq_term s3)
+        (ext_term sigma_term tau_term Eq_term s4)
+  | accinv s0 s1 s2 s3 s4 s5 s6 =>
+      congr_accinv (eq_refl s0) (ext_term sigma_term tau_term Eq_term s1)
+        (ext_term (up_term_term (up_term_term sigma_term))
+           (up_term_term (up_term_term tau_term))
+           (upExt_term_term _ _ (upExt_term_term _ _ Eq_term)) s2)
+        (ext_term sigma_term tau_term Eq_term s3)
+        (ext_term sigma_term tau_term Eq_term s4)
+        (ext_term sigma_term tau_term Eq_term s5)
+        (ext_term sigma_term tau_term Eq_term s6)
+  | accel s0 s1 s2 s3 s4 s5 s6 s7 =>
+      congr_accel (eq_refl s0) (eq_refl s1)
+        (ext_term sigma_term tau_term Eq_term s2)
+        (ext_term (up_term_term (up_term_term sigma_term))
+           (up_term_term (up_term_term tau_term))
+           (upExt_term_term _ _ (upExt_term_term _ _ Eq_term)) s3)
+        (ext_term (up_term_term sigma_term) (up_term_term tau_term)
+           (upExt_term_term _ _ Eq_term) s4)
+        (ext_term (up_term_term (up_term_term sigma_term))
+           (up_term_term (up_term_term tau_term))
+           (upExt_term_term _ _ (upExt_term_term _ _ Eq_term)) s5)
+        (ext_term sigma_term tau_term Eq_term s6)
+        (ext_term sigma_term tau_term Eq_term s7)
+  | obseq s0 s1 s2 s3 =>
+      congr_obseq (eq_refl s0) (ext_term sigma_term tau_term Eq_term s1)
+        (ext_term sigma_term tau_term Eq_term s2)
+        (ext_term sigma_term tau_term Eq_term s3)
+  | obsrefl s0 s1 s2 =>
+      congr_obsrefl (eq_refl s0) (ext_term sigma_term tau_term Eq_term s1)
+        (ext_term sigma_term tau_term Eq_term s2)
+  | J s0 s1 s2 s3 s4 s5 s6 =>
+      congr_J (eq_refl s0) (ext_term sigma_term tau_term Eq_term s1)
+        (ext_term sigma_term tau_term Eq_term s2)
+        (ext_term (up_term_term sigma_term) (up_term_term tau_term)
+           (upExt_term_term _ _ Eq_term) s3)
+        (ext_term sigma_term tau_term Eq_term s4)
+        (ext_term sigma_term tau_term Eq_term s5)
+        (ext_term sigma_term tau_term Eq_term s6)
+  | cast s0 s1 s2 s3 s4 =>
+      congr_cast (eq_refl s0) (ext_term sigma_term tau_term Eq_term s1)
+        (ext_term sigma_term tau_term Eq_term s2)
+        (ext_term sigma_term tau_term Eq_term s3)
+        (ext_term sigma_term tau_term Eq_term s4)
+  | injpi1 s0 s1 s2 s3 s4 s5 s6 =>
+      congr_injpi1 (eq_refl s0) (eq_refl s1)
+        (ext_term sigma_term tau_term Eq_term s2)
+        (ext_term sigma_term tau_term Eq_term s3)
+        (ext_term (up_term_term sigma_term) (up_term_term tau_term)
+           (upExt_term_term _ _ Eq_term) s4)
+        (ext_term (up_term_term sigma_term) (up_term_term tau_term)
+           (upExt_term_term _ _ Eq_term) s5)
+        (ext_term sigma_term tau_term Eq_term s6)
+  | injpi2 s0 s1 s2 s3 s4 s5 s6 s7 =>
+      congr_injpi2 (eq_refl s0) (eq_refl s1)
+        (ext_term sigma_term tau_term Eq_term s2)
+        (ext_term sigma_term tau_term Eq_term s3)
+        (ext_term (up_term_term sigma_term) (up_term_term tau_term)
+           (upExt_term_term _ _ Eq_term) s4)
+        (ext_term (up_term_term sigma_term) (up_term_term tau_term)
+           (upExt_term_term _ _ Eq_term) s5)
+        (ext_term sigma_term tau_term Eq_term s6)
+        (ext_term sigma_term tau_term Eq_term s7)
+  end.
+
+Lemma up_ren_ren_term_term (xi : nat -> nat) (zeta : nat -> nat)
+  (rho : nat -> nat) (Eq : forall x, funcomp zeta xi x = rho x) :
+  forall x,
+  funcomp (upRen_term_term zeta) (upRen_term_term xi) x =
+  upRen_term_term rho x.
+Proof.
+exact (up_ren_ren xi zeta rho Eq).
+Qed.
+
+Fixpoint compRenRen_term (xi_term : nat -> nat) (zeta_term : nat -> nat)
+(rho_term : nat -> nat)
+(Eq_term : forall x, funcomp zeta_term xi_term x = rho_term x) (s : term)
+{struct s} : ren_term zeta_term (ren_term xi_term s) = ren_term rho_term s :=
+  match s with
+  | var s0 => ap (var) (Eq_term s0)
+  | Sort s0 => congr_Sort (eq_refl s0)
+  | assm s0 => congr_assm (eq_refl s0)
+  | Pi s0 s1 s2 s3 =>
+      congr_Pi (eq_refl s0) (eq_refl s1)
+        (compRenRen_term xi_term zeta_term rho_term Eq_term s2)
+        (compRenRen_term (upRen_term_term xi_term)
+           (upRen_term_term zeta_term) (upRen_term_term rho_term)
+           (up_ren_ren _ _ _ Eq_term) s3)
+  | lam s0 s1 s2 s3 s4 =>
+      congr_lam (eq_refl s0) (eq_refl s1)
+        (compRenRen_term xi_term zeta_term rho_term Eq_term s2)
+        (compRenRen_term (upRen_term_term xi_term)
+           (upRen_term_term zeta_term) (upRen_term_term rho_term)
+           (up_ren_ren _ _ _ Eq_term) s3)
+        (compRenRen_term (upRen_term_term xi_term)
+           (upRen_term_term zeta_term) (upRen_term_term rho_term)
+           (up_ren_ren _ _ _ Eq_term) s4)
+  | app s0 s1 s2 s3 s4 s5 =>
+      congr_app (eq_refl s0) (eq_refl s1)
+        (compRenRen_term xi_term zeta_term rho_term Eq_term s2)
+        (compRenRen_term (upRen_term_term xi_term)
+           (upRen_term_term zeta_term) (upRen_term_term rho_term)
+           (up_ren_ren _ _ _ Eq_term) s3)
+        (compRenRen_term xi_term zeta_term rho_term Eq_term s4)
+        (compRenRen_term xi_term zeta_term rho_term Eq_term s5)
+  | Nat => congr_Nat
+  | zero => congr_zero
+  | succ s0 =>
+      congr_succ (compRenRen_term xi_term zeta_term rho_term Eq_term s0)
+  | rec s0 s1 s2 s3 s4 =>
+      congr_rec (eq_refl s0)
+        (compRenRen_term (upRen_term_term xi_term)
+           (upRen_term_term zeta_term) (upRen_term_term rho_term)
+           (up_ren_ren _ _ _ Eq_term) s1)
+        (compRenRen_term xi_term zeta_term rho_term Eq_term s2)
+        (compRenRen_term (upRen_term_term (upRen_term_term xi_term))
+           (upRen_term_term (upRen_term_term zeta_term))
+           (upRen_term_term (upRen_term_term rho_term))
+           (up_ren_ren _ _ _ (up_ren_ren _ _ _ Eq_term)) s3)
+        (compRenRen_term xi_term zeta_term rho_term Eq_term s4)
+  | acc s0 s1 s2 s3 =>
+      congr_acc (eq_refl s0)
+        (compRenRen_term xi_term zeta_term rho_term Eq_term s1)
+        (compRenRen_term (upRen_term_term (upRen_term_term xi_term))
+           (upRen_term_term (upRen_term_term zeta_term))
+           (upRen_term_term (upRen_term_term rho_term))
+           (up_ren_ren _ _ _ (up_ren_ren _ _ _ Eq_term)) s2)
+        (compRenRen_term xi_term zeta_term rho_term Eq_term s3)
+  | accin s0 s1 s2 s3 s4 =>
+      congr_accin (eq_refl s0)
+        (compRenRen_term xi_term zeta_term rho_term Eq_term s1)
+        (compRenRen_term (upRen_term_term (upRen_term_term xi_term))
+           (upRen_term_term (upRen_term_term zeta_term))
+           (upRen_term_term (upRen_term_term rho_term))
+           (up_ren_ren _ _ _ (up_ren_ren _ _ _ Eq_term)) s2)
+        (compRenRen_term xi_term zeta_term rho_term Eq_term s3)
+        (compRenRen_term xi_term zeta_term rho_term Eq_term s4)
+  | accinv s0 s1 s2 s3 s4 s5 s6 =>
+      congr_accinv (eq_refl s0)
+        (compRenRen_term xi_term zeta_term rho_term Eq_term s1)
+        (compRenRen_term (upRen_term_term (upRen_term_term xi_term))
+           (upRen_term_term (upRen_term_term zeta_term))
+           (upRen_term_term (upRen_term_term rho_term))
+           (up_ren_ren _ _ _ (up_ren_ren _ _ _ Eq_term)) s2)
+        (compRenRen_term xi_term zeta_term rho_term Eq_term s3)
+        (compRenRen_term xi_term zeta_term rho_term Eq_term s4)
+        (compRenRen_term xi_term zeta_term rho_term Eq_term s5)
+        (compRenRen_term xi_term zeta_term rho_term Eq_term s6)
+  | accel s0 s1 s2 s3 s4 s5 s6 s7 =>
+      congr_accel (eq_refl s0) (eq_refl s1)
+        (compRenRen_term xi_term zeta_term rho_term Eq_term s2)
+        (compRenRen_term (upRen_term_term (upRen_term_term xi_term))
+           (upRen_term_term (upRen_term_term zeta_term))
+           (upRen_term_term (upRen_term_term rho_term))
+           (up_ren_ren _ _ _ (up_ren_ren _ _ _ Eq_term)) s3)
+        (compRenRen_term (upRen_term_term xi_term)
+           (upRen_term_term zeta_term) (upRen_term_term rho_term)
+           (up_ren_ren _ _ _ Eq_term) s4)
+        (compRenRen_term (upRen_term_term (upRen_term_term xi_term))
+           (upRen_term_term (upRen_term_term zeta_term))
+           (upRen_term_term (upRen_term_term rho_term))
+           (up_ren_ren _ _ _ (up_ren_ren _ _ _ Eq_term)) s5)
+        (compRenRen_term xi_term zeta_term rho_term Eq_term s6)
+        (compRenRen_term xi_term zeta_term rho_term Eq_term s7)
+  | obseq s0 s1 s2 s3 =>
+      congr_obseq (eq_refl s0)
+        (compRenRen_term xi_term zeta_term rho_term Eq_term s1)
+        (compRenRen_term xi_term zeta_term rho_term Eq_term s2)
+        (compRenRen_term xi_term zeta_term rho_term Eq_term s3)
+  | obsrefl s0 s1 s2 =>
+      congr_obsrefl (eq_refl s0)
+        (compRenRen_term xi_term zeta_term rho_term Eq_term s1)
+        (compRenRen_term xi_term zeta_term rho_term Eq_term s2)
+  | J s0 s1 s2 s3 s4 s5 s6 =>
+      congr_J (eq_refl s0)
+        (compRenRen_term xi_term zeta_term rho_term Eq_term s1)
+        (compRenRen_term xi_term zeta_term rho_term Eq_term s2)
+        (compRenRen_term (upRen_term_term xi_term)
+           (upRen_term_term zeta_term) (upRen_term_term rho_term)
+           (up_ren_ren _ _ _ Eq_term) s3)
+        (compRenRen_term xi_term zeta_term rho_term Eq_term s4)
+        (compRenRen_term xi_term zeta_term rho_term Eq_term s5)
+        (compRenRen_term xi_term zeta_term rho_term Eq_term s6)
+  | cast s0 s1 s2 s3 s4 =>
+      congr_cast (eq_refl s0)
+        (compRenRen_term xi_term zeta_term rho_term Eq_term s1)
+        (compRenRen_term xi_term zeta_term rho_term Eq_term s2)
+        (compRenRen_term xi_term zeta_term rho_term Eq_term s3)
+        (compRenRen_term xi_term zeta_term rho_term Eq_term s4)
+  | injpi1 s0 s1 s2 s3 s4 s5 s6 =>
+      congr_injpi1 (eq_refl s0) (eq_refl s1)
+        (compRenRen_term xi_term zeta_term rho_term Eq_term s2)
+        (compRenRen_term xi_term zeta_term rho_term Eq_term s3)
+        (compRenRen_term (upRen_term_term xi_term)
+           (upRen_term_term zeta_term) (upRen_term_term rho_term)
+           (up_ren_ren _ _ _ Eq_term) s4)
+        (compRenRen_term (upRen_term_term xi_term)
+           (upRen_term_term zeta_term) (upRen_term_term rho_term)
+           (up_ren_ren _ _ _ Eq_term) s5)
+        (compRenRen_term xi_term zeta_term rho_term Eq_term s6)
+  | injpi2 s0 s1 s2 s3 s4 s5 s6 s7 =>
+      congr_injpi2 (eq_refl s0) (eq_refl s1)
+        (compRenRen_term xi_term zeta_term rho_term Eq_term s2)
+        (compRenRen_term xi_term zeta_term rho_term Eq_term s3)
+        (compRenRen_term (upRen_term_term xi_term)
+           (upRen_term_term zeta_term) (upRen_term_term rho_term)
+           (up_ren_ren _ _ _ Eq_term) s4)
+        (compRenRen_term (upRen_term_term xi_term)
+           (upRen_term_term zeta_term) (upRen_term_term rho_term)
+           (up_ren_ren _ _ _ Eq_term) s5)
+        (compRenRen_term xi_term zeta_term rho_term Eq_term s6)
+        (compRenRen_term xi_term zeta_term rho_term Eq_term s7)
+  end.
+
+Lemma up_ren_subst_term_term (xi : nat -> nat) (tau : nat -> term)
+  (theta : nat -> term) (Eq : forall x, funcomp tau xi x = theta x) :
+  forall x,
+  funcomp (up_term_term tau) (upRen_term_term xi) x = up_term_term theta x.
+Proof.
+exact (fun n =>
+       match n with
+       | S n' => ap (ren_term shift) (Eq n')
+       | O => eq_refl
+       end).
+Qed.
+
+Fixpoint compRenSubst_term (xi_term : nat -> nat) (tau_term : nat -> term)
+(theta_term : nat -> term)
+(Eq_term : forall x, funcomp tau_term xi_term x = theta_term x) (s : term)
+{struct s} :
+subst_term tau_term (ren_term xi_term s) = subst_term theta_term s :=
+  match s with
+  | var s0 => Eq_term s0
+  | Sort s0 => congr_Sort (eq_refl s0)
+  | assm s0 => congr_assm (eq_refl s0)
+  | Pi s0 s1 s2 s3 =>
+      congr_Pi (eq_refl s0) (eq_refl s1)
+        (compRenSubst_term xi_term tau_term theta_term Eq_term s2)
+        (compRenSubst_term (upRen_term_term xi_term) (up_term_term tau_term)
+           (up_term_term theta_term) (up_ren_subst_term_term _ _ _ Eq_term)
+           s3)
+  | lam s0 s1 s2 s3 s4 =>
+      congr_lam (eq_refl s0) (eq_refl s1)
+        (compRenSubst_term xi_term tau_term theta_term Eq_term s2)
+        (compRenSubst_term (upRen_term_term xi_term) (up_term_term tau_term)
+           (up_term_term theta_term) (up_ren_subst_term_term _ _ _ Eq_term)
+           s3)
+        (compRenSubst_term (upRen_term_term xi_term) (up_term_term tau_term)
+           (up_term_term theta_term) (up_ren_subst_term_term _ _ _ Eq_term)
+           s4)
+  | app s0 s1 s2 s3 s4 s5 =>
+      congr_app (eq_refl s0) (eq_refl s1)
+        (compRenSubst_term xi_term tau_term theta_term Eq_term s2)
+        (compRenSubst_term (upRen_term_term xi_term) (up_term_term tau_term)
+           (up_term_term theta_term) (up_ren_subst_term_term _ _ _ Eq_term)
+           s3)
+        (compRenSubst_term xi_term tau_term theta_term Eq_term s4)
+        (compRenSubst_term xi_term tau_term theta_term Eq_term s5)
+  | Nat => congr_Nat
+  | zero => congr_zero
+  | succ s0 =>
+      congr_succ (compRenSubst_term xi_term tau_term theta_term Eq_term s0)
+  | rec s0 s1 s2 s3 s4 =>
+      congr_rec (eq_refl s0)
+        (compRenSubst_term (upRen_term_term xi_term) (up_term_term tau_term)
+           (up_term_term theta_term) (up_ren_subst_term_term _ _ _ Eq_term)
+           s1)
+        (compRenSubst_term xi_term tau_term theta_term Eq_term s2)
+        (compRenSubst_term (upRen_term_term (upRen_term_term xi_term))
+           (up_term_term (up_term_term tau_term))
+           (up_term_term (up_term_term theta_term))
+           (up_ren_subst_term_term _ _ _
+              (up_ren_subst_term_term _ _ _ Eq_term))
+           s3)
+        (compRenSubst_term xi_term tau_term theta_term Eq_term s4)
+  | acc s0 s1 s2 s3 =>
+      congr_acc (eq_refl s0)
+        (compRenSubst_term xi_term tau_term theta_term Eq_term s1)
+        (compRenSubst_term (upRen_term_term (upRen_term_term xi_term))
+           (up_term_term (up_term_term tau_term))
+           (up_term_term (up_term_term theta_term))
+           (up_ren_subst_term_term _ _ _
+              (up_ren_subst_term_term _ _ _ Eq_term))
+           s2)
+        (compRenSubst_term xi_term tau_term theta_term Eq_term s3)
+  | accin s0 s1 s2 s3 s4 =>
+      congr_accin (eq_refl s0)
+        (compRenSubst_term xi_term tau_term theta_term Eq_term s1)
+        (compRenSubst_term (upRen_term_term (upRen_term_term xi_term))
+           (up_term_term (up_term_term tau_term))
+           (up_term_term (up_term_term theta_term))
+           (up_ren_subst_term_term _ _ _
+              (up_ren_subst_term_term _ _ _ Eq_term))
+           s2)
+        (compRenSubst_term xi_term tau_term theta_term Eq_term s3)
+        (compRenSubst_term xi_term tau_term theta_term Eq_term s4)
+  | accinv s0 s1 s2 s3 s4 s5 s6 =>
+      congr_accinv (eq_refl s0)
+        (compRenSubst_term xi_term tau_term theta_term Eq_term s1)
+        (compRenSubst_term (upRen_term_term (upRen_term_term xi_term))
+           (up_term_term (up_term_term tau_term))
+           (up_term_term (up_term_term theta_term))
+           (up_ren_subst_term_term _ _ _
+              (up_ren_subst_term_term _ _ _ Eq_term))
+           s2)
+        (compRenSubst_term xi_term tau_term theta_term Eq_term s3)
+        (compRenSubst_term xi_term tau_term theta_term Eq_term s4)
+        (compRenSubst_term xi_term tau_term theta_term Eq_term s5)
+        (compRenSubst_term xi_term tau_term theta_term Eq_term s6)
+  | accel s0 s1 s2 s3 s4 s5 s6 s7 =>
+      congr_accel (eq_refl s0) (eq_refl s1)
+        (compRenSubst_term xi_term tau_term theta_term Eq_term s2)
+        (compRenSubst_term (upRen_term_term (upRen_term_term xi_term))
+           (up_term_term (up_term_term tau_term))
+           (up_term_term (up_term_term theta_term))
+           (up_ren_subst_term_term _ _ _
+              (up_ren_subst_term_term _ _ _ Eq_term))
+           s3)
+        (compRenSubst_term (upRen_term_term xi_term) (up_term_term tau_term)
+           (up_term_term theta_term) (up_ren_subst_term_term _ _ _ Eq_term)
+           s4)
+        (compRenSubst_term (upRen_term_term (upRen_term_term xi_term))
+           (up_term_term (up_term_term tau_term))
+           (up_term_term (up_term_term theta_term))
+           (up_ren_subst_term_term _ _ _
+              (up_ren_subst_term_term _ _ _ Eq_term))
+           s5)
+        (compRenSubst_term xi_term tau_term theta_term Eq_term s6)
+        (compRenSubst_term xi_term tau_term theta_term Eq_term s7)
+  | obseq s0 s1 s2 s3 =>
+      congr_obseq (eq_refl s0)
+        (compRenSubst_term xi_term tau_term theta_term Eq_term s1)
+        (compRenSubst_term xi_term tau_term theta_term Eq_term s2)
+        (compRenSubst_term xi_term tau_term theta_term Eq_term s3)
+  | obsrefl s0 s1 s2 =>
+      congr_obsrefl (eq_refl s0)
+        (compRenSubst_term xi_term tau_term theta_term Eq_term s1)
+        (compRenSubst_term xi_term tau_term theta_term Eq_term s2)
+  | J s0 s1 s2 s3 s4 s5 s6 =>
+      congr_J (eq_refl s0)
+        (compRenSubst_term xi_term tau_term theta_term Eq_term s1)
+        (compRenSubst_term xi_term tau_term theta_term Eq_term s2)
+        (compRenSubst_term (upRen_term_term xi_term) (up_term_term tau_term)
+           (up_term_term theta_term) (up_ren_subst_term_term _ _ _ Eq_term)
+           s3)
+        (compRenSubst_term xi_term tau_term theta_term Eq_term s4)
+        (compRenSubst_term xi_term tau_term theta_term Eq_term s5)
+        (compRenSubst_term xi_term tau_term theta_term Eq_term s6)
+  | cast s0 s1 s2 s3 s4 =>
+      congr_cast (eq_refl s0)
+        (compRenSubst_term xi_term tau_term theta_term Eq_term s1)
+        (compRenSubst_term xi_term tau_term theta_term Eq_term s2)
+        (compRenSubst_term xi_term tau_term theta_term Eq_term s3)
+        (compRenSubst_term xi_term tau_term theta_term Eq_term s4)
+  | injpi1 s0 s1 s2 s3 s4 s5 s6 =>
+      congr_injpi1 (eq_refl s0) (eq_refl s1)
+        (compRenSubst_term xi_term tau_term theta_term Eq_term s2)
+        (compRenSubst_term xi_term tau_term theta_term Eq_term s3)
+        (compRenSubst_term (upRen_term_term xi_term) (up_term_term tau_term)
+           (up_term_term theta_term) (up_ren_subst_term_term _ _ _ Eq_term)
+           s4)
+        (compRenSubst_term (upRen_term_term xi_term) (up_term_term tau_term)
+           (up_term_term theta_term) (up_ren_subst_term_term _ _ _ Eq_term)
+           s5)
+        (compRenSubst_term xi_term tau_term theta_term Eq_term s6)
+  | injpi2 s0 s1 s2 s3 s4 s5 s6 s7 =>
+      congr_injpi2 (eq_refl s0) (eq_refl s1)
+        (compRenSubst_term xi_term tau_term theta_term Eq_term s2)
+        (compRenSubst_term xi_term tau_term theta_term Eq_term s3)
+        (compRenSubst_term (upRen_term_term xi_term) (up_term_term tau_term)
+           (up_term_term theta_term) (up_ren_subst_term_term _ _ _ Eq_term)
+           s4)
+        (compRenSubst_term (upRen_term_term xi_term) (up_term_term tau_term)
+           (up_term_term theta_term) (up_ren_subst_term_term _ _ _ Eq_term)
+           s5)
+        (compRenSubst_term xi_term tau_term theta_term Eq_term s6)
+        (compRenSubst_term xi_term tau_term theta_term Eq_term s7)
+  end.
+
+Lemma up_subst_ren_term_term (sigma : nat -> term) (zeta_term : nat -> nat)
+  (theta : nat -> term)
+  (Eq : forall x, funcomp (ren_term zeta_term) sigma x = theta x) :
+  forall x,
+  funcomp (ren_term (upRen_term_term zeta_term)) (up_term_term sigma) x =
+  up_term_term theta x.
+Proof.
+exact (fun n =>
+       match n with
+       | S n' =>
+           eq_trans
+             (compRenRen_term shift (upRen_term_term zeta_term)
+                (funcomp shift zeta_term) (fun x => eq_refl) (sigma n'))
+             (eq_trans
+                (eq_sym
+                   (compRenRen_term zeta_term shift (funcomp shift zeta_term)
+                      (fun x => eq_refl) (sigma n')))
+                (ap (ren_term shift) (Eq n')))
+       | O => eq_refl
+       end).
+Qed.
+
+Fixpoint compSubstRen_term (sigma_term : nat -> term)
+(zeta_term : nat -> nat) (theta_term : nat -> term)
+(Eq_term : forall x, funcomp (ren_term zeta_term) sigma_term x = theta_term x)
+(s : term) {struct s} :
+ren_term zeta_term (subst_term sigma_term s) = subst_term theta_term s :=
+  match s with
+  | var s0 => Eq_term s0
+  | Sort s0 => congr_Sort (eq_refl s0)
+  | assm s0 => congr_assm (eq_refl s0)
+  | Pi s0 s1 s2 s3 =>
+      congr_Pi (eq_refl s0) (eq_refl s1)
+        (compSubstRen_term sigma_term zeta_term theta_term Eq_term s2)
+        (compSubstRen_term (up_term_term sigma_term)
+           (upRen_term_term zeta_term) (up_term_term theta_term)
+           (up_subst_ren_term_term _ _ _ Eq_term) s3)
+  | lam s0 s1 s2 s3 s4 =>
+      congr_lam (eq_refl s0) (eq_refl s1)
+        (compSubstRen_term sigma_term zeta_term theta_term Eq_term s2)
+        (compSubstRen_term (up_term_term sigma_term)
+           (upRen_term_term zeta_term) (up_term_term theta_term)
+           (up_subst_ren_term_term _ _ _ Eq_term) s3)
+        (compSubstRen_term (up_term_term sigma_term)
+           (upRen_term_term zeta_term) (up_term_term theta_term)
+           (up_subst_ren_term_term _ _ _ Eq_term) s4)
+  | app s0 s1 s2 s3 s4 s5 =>
+      congr_app (eq_refl s0) (eq_refl s1)
+        (compSubstRen_term sigma_term zeta_term theta_term Eq_term s2)
+        (compSubstRen_term (up_term_term sigma_term)
+           (upRen_term_term zeta_term) (up_term_term theta_term)
+           (up_subst_ren_term_term _ _ _ Eq_term) s3)
+        (compSubstRen_term sigma_term zeta_term theta_term Eq_term s4)
+        (compSubstRen_term sigma_term zeta_term theta_term Eq_term s5)
+  | Nat => congr_Nat
+  | zero => congr_zero
+  | succ s0 =>
+      congr_succ
+        (compSubstRen_term sigma_term zeta_term theta_term Eq_term s0)
+  | rec s0 s1 s2 s3 s4 =>
+      congr_rec (eq_refl s0)
+        (compSubstRen_term (up_term_term sigma_term)
+           (upRen_term_term zeta_term) (up_term_term theta_term)
+           (up_subst_ren_term_term _ _ _ Eq_term) s1)
+        (compSubstRen_term sigma_term zeta_term theta_term Eq_term s2)
+        (compSubstRen_term (up_term_term (up_term_term sigma_term))
+           (upRen_term_term (upRen_term_term zeta_term))
+           (up_term_term (up_term_term theta_term))
+           (up_subst_ren_term_term _ _ _
+              (up_subst_ren_term_term _ _ _ Eq_term))
+           s3)
+        (compSubstRen_term sigma_term zeta_term theta_term Eq_term s4)
+  | acc s0 s1 s2 s3 =>
+      congr_acc (eq_refl s0)
+        (compSubstRen_term sigma_term zeta_term theta_term Eq_term s1)
+        (compSubstRen_term (up_term_term (up_term_term sigma_term))
+           (upRen_term_term (upRen_term_term zeta_term))
+           (up_term_term (up_term_term theta_term))
+           (up_subst_ren_term_term _ _ _
+              (up_subst_ren_term_term _ _ _ Eq_term))
+           s2)
+        (compSubstRen_term sigma_term zeta_term theta_term Eq_term s3)
+  | accin s0 s1 s2 s3 s4 =>
+      congr_accin (eq_refl s0)
+        (compSubstRen_term sigma_term zeta_term theta_term Eq_term s1)
+        (compSubstRen_term (up_term_term (up_term_term sigma_term))
+           (upRen_term_term (upRen_term_term zeta_term))
+           (up_term_term (up_term_term theta_term))
+           (up_subst_ren_term_term _ _ _
+              (up_subst_ren_term_term _ _ _ Eq_term))
+           s2)
+        (compSubstRen_term sigma_term zeta_term theta_term Eq_term s3)
+        (compSubstRen_term sigma_term zeta_term theta_term Eq_term s4)
+  | accinv s0 s1 s2 s3 s4 s5 s6 =>
+      congr_accinv (eq_refl s0)
+        (compSubstRen_term sigma_term zeta_term theta_term Eq_term s1)
+        (compSubstRen_term (up_term_term (up_term_term sigma_term))
+           (upRen_term_term (upRen_term_term zeta_term))
+           (up_term_term (up_term_term theta_term))
+           (up_subst_ren_term_term _ _ _
+              (up_subst_ren_term_term _ _ _ Eq_term))
+           s2)
+        (compSubstRen_term sigma_term zeta_term theta_term Eq_term s3)
+        (compSubstRen_term sigma_term zeta_term theta_term Eq_term s4)
+        (compSubstRen_term sigma_term zeta_term theta_term Eq_term s5)
+        (compSubstRen_term sigma_term zeta_term theta_term Eq_term s6)
+  | accel s0 s1 s2 s3 s4 s5 s6 s7 =>
+      congr_accel (eq_refl s0) (eq_refl s1)
+        (compSubstRen_term sigma_term zeta_term theta_term Eq_term s2)
+        (compSubstRen_term (up_term_term (up_term_term sigma_term))
+           (upRen_term_term (upRen_term_term zeta_term))
+           (up_term_term (up_term_term theta_term))
+           (up_subst_ren_term_term _ _ _
+              (up_subst_ren_term_term _ _ _ Eq_term))
+           s3)
+        (compSubstRen_term (up_term_term sigma_term)
+           (upRen_term_term zeta_term) (up_term_term theta_term)
+           (up_subst_ren_term_term _ _ _ Eq_term) s4)
+        (compSubstRen_term (up_term_term (up_term_term sigma_term))
+           (upRen_term_term (upRen_term_term zeta_term))
+           (up_term_term (up_term_term theta_term))
+           (up_subst_ren_term_term _ _ _
+              (up_subst_ren_term_term _ _ _ Eq_term))
+           s5)
+        (compSubstRen_term sigma_term zeta_term theta_term Eq_term s6)
+        (compSubstRen_term sigma_term zeta_term theta_term Eq_term s7)
+  | obseq s0 s1 s2 s3 =>
+      congr_obseq (eq_refl s0)
+        (compSubstRen_term sigma_term zeta_term theta_term Eq_term s1)
+        (compSubstRen_term sigma_term zeta_term theta_term Eq_term s2)
+        (compSubstRen_term sigma_term zeta_term theta_term Eq_term s3)
+  | obsrefl s0 s1 s2 =>
+      congr_obsrefl (eq_refl s0)
+        (compSubstRen_term sigma_term zeta_term theta_term Eq_term s1)
+        (compSubstRen_term sigma_term zeta_term theta_term Eq_term s2)
+  | J s0 s1 s2 s3 s4 s5 s6 =>
+      congr_J (eq_refl s0)
+        (compSubstRen_term sigma_term zeta_term theta_term Eq_term s1)
+        (compSubstRen_term sigma_term zeta_term theta_term Eq_term s2)
+        (compSubstRen_term (up_term_term sigma_term)
+           (upRen_term_term zeta_term) (up_term_term theta_term)
+           (up_subst_ren_term_term _ _ _ Eq_term) s3)
+        (compSubstRen_term sigma_term zeta_term theta_term Eq_term s4)
+        (compSubstRen_term sigma_term zeta_term theta_term Eq_term s5)
+        (compSubstRen_term sigma_term zeta_term theta_term Eq_term s6)
+  | cast s0 s1 s2 s3 s4 =>
+      congr_cast (eq_refl s0)
+        (compSubstRen_term sigma_term zeta_term theta_term Eq_term s1)
+        (compSubstRen_term sigma_term zeta_term theta_term Eq_term s2)
+        (compSubstRen_term sigma_term zeta_term theta_term Eq_term s3)
+        (compSubstRen_term sigma_term zeta_term theta_term Eq_term s4)
+  | injpi1 s0 s1 s2 s3 s4 s5 s6 =>
+      congr_injpi1 (eq_refl s0) (eq_refl s1)
+        (compSubstRen_term sigma_term zeta_term theta_term Eq_term s2)
+        (compSubstRen_term sigma_term zeta_term theta_term Eq_term s3)
+        (compSubstRen_term (up_term_term sigma_term)
+           (upRen_term_term zeta_term) (up_term_term theta_term)
+           (up_subst_ren_term_term _ _ _ Eq_term) s4)
+        (compSubstRen_term (up_term_term sigma_term)
+           (upRen_term_term zeta_term) (up_term_term theta_term)
+           (up_subst_ren_term_term _ _ _ Eq_term) s5)
+        (compSubstRen_term sigma_term zeta_term theta_term Eq_term s6)
+  | injpi2 s0 s1 s2 s3 s4 s5 s6 s7 =>
+      congr_injpi2 (eq_refl s0) (eq_refl s1)
+        (compSubstRen_term sigma_term zeta_term theta_term Eq_term s2)
+        (compSubstRen_term sigma_term zeta_term theta_term Eq_term s3)
+        (compSubstRen_term (up_term_term sigma_term)
+           (upRen_term_term zeta_term) (up_term_term theta_term)
+           (up_subst_ren_term_term _ _ _ Eq_term) s4)
+        (compSubstRen_term (up_term_term sigma_term)
+           (upRen_term_term zeta_term) (up_term_term theta_term)
+           (up_subst_ren_term_term _ _ _ Eq_term) s5)
+        (compSubstRen_term sigma_term zeta_term theta_term Eq_term s6)
+        (compSubstRen_term sigma_term zeta_term theta_term Eq_term s7)
+  end.
+
+Lemma up_subst_subst_term_term (sigma : nat -> term) (tau_term : nat -> term)
+  (theta : nat -> term)
+  (Eq : forall x, funcomp (subst_term tau_term) sigma x = theta x) :
+  forall x,
+  funcomp (subst_term (up_term_term tau_term)) (up_term_term sigma) x =
+  up_term_term theta x.
+Proof.
+exact (fun n =>
+       match n with
+       | S n' =>
+           eq_trans
+             (compRenSubst_term shift (up_term_term tau_term)
+                (funcomp (up_term_term tau_term) shift) (fun x => eq_refl)
+                (sigma n'))
+             (eq_trans
+                (eq_sym
+                   (compSubstRen_term tau_term shift
+                      (funcomp (ren_term shift) tau_term) (fun x => eq_refl)
+                      (sigma n')))
+                (ap (ren_term shift) (Eq n')))
+       | O => eq_refl
+       end).
+Qed.
+
+Fixpoint compSubstSubst_term (sigma_term : nat -> term)
+(tau_term : nat -> term) (theta_term : nat -> term)
+(Eq_term : forall x,
+           funcomp (subst_term tau_term) sigma_term x = theta_term x)
+(s : term) {struct s} :
+subst_term tau_term (subst_term sigma_term s) = subst_term theta_term s :=
+  match s with
+  | var s0 => Eq_term s0
+  | Sort s0 => congr_Sort (eq_refl s0)
+  | assm s0 => congr_assm (eq_refl s0)
+  | Pi s0 s1 s2 s3 =>
+      congr_Pi (eq_refl s0) (eq_refl s1)
+        (compSubstSubst_term sigma_term tau_term theta_term Eq_term s2)
+        (compSubstSubst_term (up_term_term sigma_term)
+           (up_term_term tau_term) (up_term_term theta_term)
+           (up_subst_subst_term_term _ _ _ Eq_term) s3)
+  | lam s0 s1 s2 s3 s4 =>
+      congr_lam (eq_refl s0) (eq_refl s1)
+        (compSubstSubst_term sigma_term tau_term theta_term Eq_term s2)
+        (compSubstSubst_term (up_term_term sigma_term)
+           (up_term_term tau_term) (up_term_term theta_term)
+           (up_subst_subst_term_term _ _ _ Eq_term) s3)
+        (compSubstSubst_term (up_term_term sigma_term)
+           (up_term_term tau_term) (up_term_term theta_term)
+           (up_subst_subst_term_term _ _ _ Eq_term) s4)
+  | app s0 s1 s2 s3 s4 s5 =>
+      congr_app (eq_refl s0) (eq_refl s1)
+        (compSubstSubst_term sigma_term tau_term theta_term Eq_term s2)
+        (compSubstSubst_term (up_term_term sigma_term)
+           (up_term_term tau_term) (up_term_term theta_term)
+           (up_subst_subst_term_term _ _ _ Eq_term) s3)
+        (compSubstSubst_term sigma_term tau_term theta_term Eq_term s4)
+        (compSubstSubst_term sigma_term tau_term theta_term Eq_term s5)
+  | Nat => congr_Nat
+  | zero => congr_zero
+  | succ s0 =>
+      congr_succ
+        (compSubstSubst_term sigma_term tau_term theta_term Eq_term s0)
+  | rec s0 s1 s2 s3 s4 =>
+      congr_rec (eq_refl s0)
+        (compSubstSubst_term (up_term_term sigma_term)
+           (up_term_term tau_term) (up_term_term theta_term)
+           (up_subst_subst_term_term _ _ _ Eq_term) s1)
+        (compSubstSubst_term sigma_term tau_term theta_term Eq_term s2)
+        (compSubstSubst_term (up_term_term (up_term_term sigma_term))
+           (up_term_term (up_term_term tau_term))
+           (up_term_term (up_term_term theta_term))
+           (up_subst_subst_term_term _ _ _
+              (up_subst_subst_term_term _ _ _ Eq_term))
+           s3)
+        (compSubstSubst_term sigma_term tau_term theta_term Eq_term s4)
+  | acc s0 s1 s2 s3 =>
+      congr_acc (eq_refl s0)
+        (compSubstSubst_term sigma_term tau_term theta_term Eq_term s1)
+        (compSubstSubst_term (up_term_term (up_term_term sigma_term))
+           (up_term_term (up_term_term tau_term))
+           (up_term_term (up_term_term theta_term))
+           (up_subst_subst_term_term _ _ _
+              (up_subst_subst_term_term _ _ _ Eq_term))
+           s2)
+        (compSubstSubst_term sigma_term tau_term theta_term Eq_term s3)
+  | accin s0 s1 s2 s3 s4 =>
+      congr_accin (eq_refl s0)
+        (compSubstSubst_term sigma_term tau_term theta_term Eq_term s1)
+        (compSubstSubst_term (up_term_term (up_term_term sigma_term))
+           (up_term_term (up_term_term tau_term))
+           (up_term_term (up_term_term theta_term))
+           (up_subst_subst_term_term _ _ _
+              (up_subst_subst_term_term _ _ _ Eq_term))
+           s2)
+        (compSubstSubst_term sigma_term tau_term theta_term Eq_term s3)
+        (compSubstSubst_term sigma_term tau_term theta_term Eq_term s4)
+  | accinv s0 s1 s2 s3 s4 s5 s6 =>
+      congr_accinv (eq_refl s0)
+        (compSubstSubst_term sigma_term tau_term theta_term Eq_term s1)
+        (compSubstSubst_term (up_term_term (up_term_term sigma_term))
+           (up_term_term (up_term_term tau_term))
+           (up_term_term (up_term_term theta_term))
+           (up_subst_subst_term_term _ _ _
+              (up_subst_subst_term_term _ _ _ Eq_term))
+           s2)
+        (compSubstSubst_term sigma_term tau_term theta_term Eq_term s3)
+        (compSubstSubst_term sigma_term tau_term theta_term Eq_term s4)
+        (compSubstSubst_term sigma_term tau_term theta_term Eq_term s5)
+        (compSubstSubst_term sigma_term tau_term theta_term Eq_term s6)
+  | accel s0 s1 s2 s3 s4 s5 s6 s7 =>
+      congr_accel (eq_refl s0) (eq_refl s1)
+        (compSubstSubst_term sigma_term tau_term theta_term Eq_term s2)
+        (compSubstSubst_term (up_term_term (up_term_term sigma_term))
+           (up_term_term (up_term_term tau_term))
+           (up_term_term (up_term_term theta_term))
+           (up_subst_subst_term_term _ _ _
+              (up_subst_subst_term_term _ _ _ Eq_term))
+           s3)
+        (compSubstSubst_term (up_term_term sigma_term)
+           (up_term_term tau_term) (up_term_term theta_term)
+           (up_subst_subst_term_term _ _ _ Eq_term) s4)
+        (compSubstSubst_term (up_term_term (up_term_term sigma_term))
+           (up_term_term (up_term_term tau_term))
+           (up_term_term (up_term_term theta_term))
+           (up_subst_subst_term_term _ _ _
+              (up_subst_subst_term_term _ _ _ Eq_term))
+           s5)
+        (compSubstSubst_term sigma_term tau_term theta_term Eq_term s6)
+        (compSubstSubst_term sigma_term tau_term theta_term Eq_term s7)
+  | obseq s0 s1 s2 s3 =>
+      congr_obseq (eq_refl s0)
+        (compSubstSubst_term sigma_term tau_term theta_term Eq_term s1)
+        (compSubstSubst_term sigma_term tau_term theta_term Eq_term s2)
+        (compSubstSubst_term sigma_term tau_term theta_term Eq_term s3)
+  | obsrefl s0 s1 s2 =>
+      congr_obsrefl (eq_refl s0)
+        (compSubstSubst_term sigma_term tau_term theta_term Eq_term s1)
+        (compSubstSubst_term sigma_term tau_term theta_term Eq_term s2)
+  | J s0 s1 s2 s3 s4 s5 s6 =>
+      congr_J (eq_refl s0)
+        (compSubstSubst_term sigma_term tau_term theta_term Eq_term s1)
+        (compSubstSubst_term sigma_term tau_term theta_term Eq_term s2)
+        (compSubstSubst_term (up_term_term sigma_term)
+           (up_term_term tau_term) (up_term_term theta_term)
+           (up_subst_subst_term_term _ _ _ Eq_term) s3)
+        (compSubstSubst_term sigma_term tau_term theta_term Eq_term s4)
+        (compSubstSubst_term sigma_term tau_term theta_term Eq_term s5)
+        (compSubstSubst_term sigma_term tau_term theta_term Eq_term s6)
+  | cast s0 s1 s2 s3 s4 =>
+      congr_cast (eq_refl s0)
+        (compSubstSubst_term sigma_term tau_term theta_term Eq_term s1)
+        (compSubstSubst_term sigma_term tau_term theta_term Eq_term s2)
+        (compSubstSubst_term sigma_term tau_term theta_term Eq_term s3)
+        (compSubstSubst_term sigma_term tau_term theta_term Eq_term s4)
+  | injpi1 s0 s1 s2 s3 s4 s5 s6 =>
+      congr_injpi1 (eq_refl s0) (eq_refl s1)
+        (compSubstSubst_term sigma_term tau_term theta_term Eq_term s2)
+        (compSubstSubst_term sigma_term tau_term theta_term Eq_term s3)
+        (compSubstSubst_term (up_term_term sigma_term)
+           (up_term_term tau_term) (up_term_term theta_term)
+           (up_subst_subst_term_term _ _ _ Eq_term) s4)
+        (compSubstSubst_term (up_term_term sigma_term)
+           (up_term_term tau_term) (up_term_term theta_term)
+           (up_subst_subst_term_term _ _ _ Eq_term) s5)
+        (compSubstSubst_term sigma_term tau_term theta_term Eq_term s6)
+  | injpi2 s0 s1 s2 s3 s4 s5 s6 s7 =>
+      congr_injpi2 (eq_refl s0) (eq_refl s1)
+        (compSubstSubst_term sigma_term tau_term theta_term Eq_term s2)
+        (compSubstSubst_term sigma_term tau_term theta_term Eq_term s3)
+        (compSubstSubst_term (up_term_term sigma_term)
+           (up_term_term tau_term) (up_term_term theta_term)
+           (up_subst_subst_term_term _ _ _ Eq_term) s4)
+        (compSubstSubst_term (up_term_term sigma_term)
+           (up_term_term tau_term) (up_term_term theta_term)
+           (up_subst_subst_term_term _ _ _ Eq_term) s5)
+        (compSubstSubst_term sigma_term tau_term theta_term Eq_term s6)
+        (compSubstSubst_term sigma_term tau_term theta_term Eq_term s7)
+  end.
+
+Lemma renRen_term (xi_term : nat -> nat) (zeta_term : nat -> nat) (s : term)
+  :
+  ren_term zeta_term (ren_term xi_term s) =
+  ren_term (funcomp zeta_term xi_term) s.
+Proof.
+exact (compRenRen_term xi_term zeta_term _ (fun n => eq_refl) s).
+Qed.
+
+Lemma renRen'_term_pointwise (xi_term : nat -> nat) (zeta_term : nat -> nat)
+  :
+  pointwise_relation _ eq (funcomp (ren_term zeta_term) (ren_term xi_term))
+    (ren_term (funcomp zeta_term xi_term)).
+Proof.
+exact (fun s => compRenRen_term xi_term zeta_term _ (fun n => eq_refl) s).
+Qed.
+
+Lemma renSubst_term (xi_term : nat -> nat) (tau_term : nat -> term)
+  (s : term) :
+  subst_term tau_term (ren_term xi_term s) =
+  subst_term (funcomp tau_term xi_term) s.
+Proof.
+exact (compRenSubst_term xi_term tau_term _ (fun n => eq_refl) s).
+Qed.
+
+Lemma renSubst_term_pointwise (xi_term : nat -> nat) (tau_term : nat -> term)
+  :
+  pointwise_relation _ eq (funcomp (subst_term tau_term) (ren_term xi_term))
+    (subst_term (funcomp tau_term xi_term)).
+Proof.
+exact (fun s => compRenSubst_term xi_term tau_term _ (fun n => eq_refl) s).
+Qed.
+
+Lemma substRen_term (sigma_term : nat -> term) (zeta_term : nat -> nat)
+  (s : term) :
+  ren_term zeta_term (subst_term sigma_term s) =
+  subst_term (funcomp (ren_term zeta_term) sigma_term) s.
+Proof.
+exact (compSubstRen_term sigma_term zeta_term _ (fun n => eq_refl) s).
+Qed.
+
+Lemma substRen_term_pointwise (sigma_term : nat -> term)
+  (zeta_term : nat -> nat) :
+  pointwise_relation _ eq
+    (funcomp (ren_term zeta_term) (subst_term sigma_term))
+    (subst_term (funcomp (ren_term zeta_term) sigma_term)).
+Proof.
+exact (fun s => compSubstRen_term sigma_term zeta_term _ (fun n => eq_refl) s).
+Qed.
+
+Lemma substSubst_term (sigma_term : nat -> term) (tau_term : nat -> term)
+  (s : term) :
+  subst_term tau_term (subst_term sigma_term s) =
+  subst_term (funcomp (subst_term tau_term) sigma_term) s.
+Proof.
+exact (compSubstSubst_term sigma_term tau_term _ (fun n => eq_refl) s).
+Qed.
+
+Lemma substSubst_term_pointwise (sigma_term : nat -> term)
+  (tau_term : nat -> term) :
+  pointwise_relation _ eq
+    (funcomp (subst_term tau_term) (subst_term sigma_term))
+    (subst_term (funcomp (subst_term tau_term) sigma_term)).
+Proof.
+exact (fun s =>
+       compSubstSubst_term sigma_term tau_term _ (fun n => eq_refl) s).
+Qed.
+
+Lemma rinstInst_up_term_term (xi : nat -> nat) (sigma : nat -> term)
+  (Eq : forall x, funcomp (var) xi x = sigma x) :
+  forall x, funcomp (var) (upRen_term_term xi) x = up_term_term sigma x.
+Proof.
+exact (fun n =>
+       match n with
+       | S n' => ap (ren_term shift) (Eq n')
+       | O => eq_refl
+       end).
+Qed.
+
+Fixpoint rinst_inst_term (xi_term : nat -> nat) (sigma_term : nat -> term)
+(Eq_term : forall x, funcomp (var) xi_term x = sigma_term x) (s : term)
+{struct s} : ren_term xi_term s = subst_term sigma_term s :=
+  match s with
+  | var s0 => Eq_term s0
+  | Sort s0 => congr_Sort (eq_refl s0)
+  | assm s0 => congr_assm (eq_refl s0)
+  | Pi s0 s1 s2 s3 =>
+      congr_Pi (eq_refl s0) (eq_refl s1)
+        (rinst_inst_term xi_term sigma_term Eq_term s2)
+        (rinst_inst_term (upRen_term_term xi_term) (up_term_term sigma_term)
+           (rinstInst_up_term_term _ _ Eq_term) s3)
+  | lam s0 s1 s2 s3 s4 =>
+      congr_lam (eq_refl s0) (eq_refl s1)
+        (rinst_inst_term xi_term sigma_term Eq_term s2)
+        (rinst_inst_term (upRen_term_term xi_term) (up_term_term sigma_term)
+           (rinstInst_up_term_term _ _ Eq_term) s3)
+        (rinst_inst_term (upRen_term_term xi_term) (up_term_term sigma_term)
+           (rinstInst_up_term_term _ _ Eq_term) s4)
+  | app s0 s1 s2 s3 s4 s5 =>
+      congr_app (eq_refl s0) (eq_refl s1)
+        (rinst_inst_term xi_term sigma_term Eq_term s2)
+        (rinst_inst_term (upRen_term_term xi_term) (up_term_term sigma_term)
+           (rinstInst_up_term_term _ _ Eq_term) s3)
+        (rinst_inst_term xi_term sigma_term Eq_term s4)
+        (rinst_inst_term xi_term sigma_term Eq_term s5)
+  | Nat => congr_Nat
+  | zero => congr_zero
+  | succ s0 => congr_succ (rinst_inst_term xi_term sigma_term Eq_term s0)
+  | rec s0 s1 s2 s3 s4 =>
+      congr_rec (eq_refl s0)
+        (rinst_inst_term (upRen_term_term xi_term) (up_term_term sigma_term)
+           (rinstInst_up_term_term _ _ Eq_term) s1)
+        (rinst_inst_term xi_term sigma_term Eq_term s2)
+        (rinst_inst_term (upRen_term_term (upRen_term_term xi_term))
+           (up_term_term (up_term_term sigma_term))
+           (rinstInst_up_term_term _ _ (rinstInst_up_term_term _ _ Eq_term))
+           s3)
+        (rinst_inst_term xi_term sigma_term Eq_term s4)
+  | acc s0 s1 s2 s3 =>
+      congr_acc (eq_refl s0) (rinst_inst_term xi_term sigma_term Eq_term s1)
+        (rinst_inst_term (upRen_term_term (upRen_term_term xi_term))
+           (up_term_term (up_term_term sigma_term))
+           (rinstInst_up_term_term _ _ (rinstInst_up_term_term _ _ Eq_term))
+           s2)
+        (rinst_inst_term xi_term sigma_term Eq_term s3)
+  | accin s0 s1 s2 s3 s4 =>
+      congr_accin (eq_refl s0)
+        (rinst_inst_term xi_term sigma_term Eq_term s1)
+        (rinst_inst_term (upRen_term_term (upRen_term_term xi_term))
+           (up_term_term (up_term_term sigma_term))
+           (rinstInst_up_term_term _ _ (rinstInst_up_term_term _ _ Eq_term))
+           s2)
+        (rinst_inst_term xi_term sigma_term Eq_term s3)
+        (rinst_inst_term xi_term sigma_term Eq_term s4)
+  | accinv s0 s1 s2 s3 s4 s5 s6 =>
+      congr_accinv (eq_refl s0)
+        (rinst_inst_term xi_term sigma_term Eq_term s1)
+        (rinst_inst_term (upRen_term_term (upRen_term_term xi_term))
+           (up_term_term (up_term_term sigma_term))
+           (rinstInst_up_term_term _ _ (rinstInst_up_term_term _ _ Eq_term))
+           s2)
+        (rinst_inst_term xi_term sigma_term Eq_term s3)
+        (rinst_inst_term xi_term sigma_term Eq_term s4)
+        (rinst_inst_term xi_term sigma_term Eq_term s5)
+        (rinst_inst_term xi_term sigma_term Eq_term s6)
+  | accel s0 s1 s2 s3 s4 s5 s6 s7 =>
+      congr_accel (eq_refl s0) (eq_refl s1)
+        (rinst_inst_term xi_term sigma_term Eq_term s2)
+        (rinst_inst_term (upRen_term_term (upRen_term_term xi_term))
+           (up_term_term (up_term_term sigma_term))
+           (rinstInst_up_term_term _ _ (rinstInst_up_term_term _ _ Eq_term))
+           s3)
+        (rinst_inst_term (upRen_term_term xi_term) (up_term_term sigma_term)
+           (rinstInst_up_term_term _ _ Eq_term) s4)
+        (rinst_inst_term (upRen_term_term (upRen_term_term xi_term))
+           (up_term_term (up_term_term sigma_term))
+           (rinstInst_up_term_term _ _ (rinstInst_up_term_term _ _ Eq_term))
+           s5)
+        (rinst_inst_term xi_term sigma_term Eq_term s6)
+        (rinst_inst_term xi_term sigma_term Eq_term s7)
+  | obseq s0 s1 s2 s3 =>
+      congr_obseq (eq_refl s0)
+        (rinst_inst_term xi_term sigma_term Eq_term s1)
+        (rinst_inst_term xi_term sigma_term Eq_term s2)
+        (rinst_inst_term xi_term sigma_term Eq_term s3)
+  | obsrefl s0 s1 s2 =>
+      congr_obsrefl (eq_refl s0)
+        (rinst_inst_term xi_term sigma_term Eq_term s1)
+        (rinst_inst_term xi_term sigma_term Eq_term s2)
+  | J s0 s1 s2 s3 s4 s5 s6 =>
+      congr_J (eq_refl s0) (rinst_inst_term xi_term sigma_term Eq_term s1)
+        (rinst_inst_term xi_term sigma_term Eq_term s2)
+        (rinst_inst_term (upRen_term_term xi_term) (up_term_term sigma_term)
+           (rinstInst_up_term_term _ _ Eq_term) s3)
+        (rinst_inst_term xi_term sigma_term Eq_term s4)
+        (rinst_inst_term xi_term sigma_term Eq_term s5)
+        (rinst_inst_term xi_term sigma_term Eq_term s6)
+  | cast s0 s1 s2 s3 s4 =>
+      congr_cast (eq_refl s0) (rinst_inst_term xi_term sigma_term Eq_term s1)
+        (rinst_inst_term xi_term sigma_term Eq_term s2)
+        (rinst_inst_term xi_term sigma_term Eq_term s3)
+        (rinst_inst_term xi_term sigma_term Eq_term s4)
+  | injpi1 s0 s1 s2 s3 s4 s5 s6 =>
+      congr_injpi1 (eq_refl s0) (eq_refl s1)
+        (rinst_inst_term xi_term sigma_term Eq_term s2)
+        (rinst_inst_term xi_term sigma_term Eq_term s3)
+        (rinst_inst_term (upRen_term_term xi_term) (up_term_term sigma_term)
+           (rinstInst_up_term_term _ _ Eq_term) s4)
+        (rinst_inst_term (upRen_term_term xi_term) (up_term_term sigma_term)
+           (rinstInst_up_term_term _ _ Eq_term) s5)
+        (rinst_inst_term xi_term sigma_term Eq_term s6)
+  | injpi2 s0 s1 s2 s3 s4 s5 s6 s7 =>
+      congr_injpi2 (eq_refl s0) (eq_refl s1)
+        (rinst_inst_term xi_term sigma_term Eq_term s2)
+        (rinst_inst_term xi_term sigma_term Eq_term s3)
+        (rinst_inst_term (upRen_term_term xi_term) (up_term_term sigma_term)
+           (rinstInst_up_term_term _ _ Eq_term) s4)
+        (rinst_inst_term (upRen_term_term xi_term) (up_term_term sigma_term)
+           (rinstInst_up_term_term _ _ Eq_term) s5)
+        (rinst_inst_term xi_term sigma_term Eq_term s6)
+        (rinst_inst_term xi_term sigma_term Eq_term s7)
+  end.
+
+Lemma rinstInst'_term (xi_term : nat -> nat) (s : term) :
+  ren_term xi_term s = subst_term (funcomp (var) xi_term) s.
+Proof.
+exact (rinst_inst_term xi_term _ (fun n => eq_refl) s).
+Qed.
+
+Lemma rinstInst'_term_pointwise (xi_term : nat -> nat) :
+  pointwise_relation _ eq (ren_term xi_term)
+    (subst_term (funcomp (var) xi_term)).
+Proof.
+exact (fun s => rinst_inst_term xi_term _ (fun n => eq_refl) s).
+Qed.
+
+Lemma instId'_term (s : term) : subst_term (var) s = s.
+Proof.
+exact (idSubst_term (var) (fun n => eq_refl) s).
+Qed.
+
+Lemma instId'_term_pointwise : pointwise_relation _ eq (subst_term (var)) id.
+Proof.
+exact (fun s => idSubst_term (var) (fun n => eq_refl) s).
+Qed.
+
+Lemma rinstId'_term (s : term) : ren_term id s = s.
+Proof.
+exact (eq_ind_r (fun t => t = s) (instId'_term s) (rinstInst'_term id s)).
+Qed.
+
+Lemma rinstId'_term_pointwise : pointwise_relation _ eq (@ren_term id) id.
+Proof.
+exact (fun s =>
+       eq_ind_r (fun t => t = s) (instId'_term s) (rinstInst'_term id s)).
+Qed.
+
+Lemma varL'_term (sigma_term : nat -> term) (x : nat) :
+  subst_term sigma_term (var x) = sigma_term x.
+Proof.
+exact (eq_refl).
+Qed.
+
+Lemma varL'_term_pointwise (sigma_term : nat -> term) :
+  pointwise_relation _ eq (funcomp (subst_term sigma_term) (var)) sigma_term.
+Proof.
+exact (fun x => eq_refl).
+Qed.
+
+Lemma varLRen'_term (xi_term : nat -> nat) (x : nat) :
+  ren_term xi_term (var x) = var (xi_term x).
+Proof.
+exact (eq_refl).
+Qed.
+
+Lemma varLRen'_term_pointwise (xi_term : nat -> nat) :
+  pointwise_relation _ eq (funcomp (ren_term xi_term) (var))
+    (funcomp (var) xi_term).
+Proof.
+exact (fun x => eq_refl).
+Qed.
+
+Class Up_term X Y :=
+    up_term : X -> Y.
+
+#[global] Instance Subst_term : (Subst1 _ _ _) := @subst_term.
+
+#[global] Instance Up_term_term : (Up_term _ _) := @up_term_term.
+
+#[global] Instance Ren_term : (Ren1 _ _ _) := @ren_term.
+
+#[global]
+Instance VarInstance_term : (Var _ _) := @var.
+
+Notation "s [ sigma_term ]" := (subst_term sigma_term s)
+( at level 7, left associativity, only printing)  : subst_scope.
+
+Notation "↑__term" := up_term (only printing)  : subst_scope.
+
+Notation "↑__term" := up_term_term (only printing)  : subst_scope.
+
+Notation "s ⟨ xi_term ⟩" := (ren_term xi_term s)
+( at level 7, left associativity, only printing)  : subst_scope.
+
+Notation "'var'" := var ( at level 1, only printing)  : subst_scope.
+
+Notation "x '__term'" := (@ids _ _ VarInstance_term x)
+( at level 5, format "x __term", only printing)  : subst_scope.
+
+Notation "x '__term'" := (var x) ( at level 5, format "x __term")  :
+subst_scope.
+
+#[global]
+Instance subst_term_morphism :
+ (Proper (respectful (pointwise_relation _ eq) (respectful eq eq))
+    (@subst_term)).
+Proof.
+exact (fun f_term g_term Eq_term s t Eq_st =>
+       eq_ind s (fun t' => subst_term f_term s = subst_term g_term t')
+         (ext_term f_term g_term Eq_term s) t Eq_st).
+Qed.
+
+#[global]
+Instance subst_term_morphism2 :
+ (Proper (respectful (pointwise_relation _ eq) (pointwise_relation _ eq))
+    (@subst_term)).
+Proof.
+exact (fun f_term g_term Eq_term s => ext_term f_term g_term Eq_term s).
+Qed.
+
+#[global]
+Instance ren_term_morphism :
+ (Proper (respectful (pointwise_relation _ eq) (respectful eq eq))
+    (@ren_term)).
+Proof.
+exact (fun f_term g_term Eq_term s t Eq_st =>
+       eq_ind s (fun t' => ren_term f_term s = ren_term g_term t')
+         (extRen_term f_term g_term Eq_term s) t Eq_st).
+Qed.
+
+#[global]
+Instance ren_term_morphism2 :
+ (Proper (respectful (pointwise_relation _ eq) (pointwise_relation _ eq))
+    (@ren_term)).
+Proof.
+exact (fun f_term g_term Eq_term s => extRen_term f_term g_term Eq_term s).
+Qed.
+
+Ltac auto_unfold := repeat
+                     unfold VarInstance_term, Var, ids, Ren_term, Ren1, ren1,
+                      Up_term_term, Up_term, up_term, Subst_term, Subst1,
+                      subst1.
+
+Tactic Notation "auto_unfold" "in" "*" := repeat
+                                           unfold VarInstance_term, Var, ids,
+                                            Ren_term, Ren1, ren1,
+                                            Up_term_term, Up_term, up_term,
+                                            Subst_term, Subst1, subst1 
+                                            in *.
+
+Ltac asimpl' := repeat (first
+                 [ progress setoid_rewrite substSubst_term_pointwise
+                 | progress setoid_rewrite substSubst_term
+                 | progress setoid_rewrite substRen_term_pointwise
+                 | progress setoid_rewrite substRen_term
+                 | progress setoid_rewrite renSubst_term_pointwise
+                 | progress setoid_rewrite renSubst_term
+                 | progress setoid_rewrite renRen'_term_pointwise
+                 | progress setoid_rewrite renRen_term
+                 | progress setoid_rewrite varLRen'_term_pointwise
+                 | progress setoid_rewrite varLRen'_term
+                 | progress setoid_rewrite varL'_term_pointwise
+                 | progress setoid_rewrite varL'_term
+                 | progress setoid_rewrite rinstId'_term_pointwise
+                 | progress setoid_rewrite rinstId'_term
+                 | progress setoid_rewrite instId'_term_pointwise
+                 | progress setoid_rewrite instId'_term
+                 | progress unfold up_term_term, upRen_term_term, up_ren
+                 | progress cbn[subst_term ren_term]
+                 | progress fsimpl ]).
+
+Ltac asimpl := check_no_evars;
+                repeat
+                 unfold VarInstance_term, Var, ids, Ren_term, Ren1, ren1,
+                  Up_term_term, Up_term, up_term, Subst_term, Subst1, subst1
+                  in *;
+                asimpl'; minimize.
+
+Tactic Notation "asimpl" "in" hyp(J) := revert J; asimpl; intros J.
+
+Tactic Notation "auto_case" := auto_case ltac:(asimpl; cbn; eauto).
+
+Ltac substify := auto_unfold; try setoid_rewrite rinstInst'_term_pointwise;
+                  try setoid_rewrite rinstInst'_term.
+
+Ltac renamify := auto_unfold;
+                  try setoid_rewrite_left rinstInst'_term_pointwise;
+                  try setoid_rewrite_left rinstInst'_term.
+
+End Core.
+
+Module Extra.
+
+Import Core.
+
+#[global] Hint Opaque subst_term: rewrite.
+
+#[global] Hint Opaque ren_term: rewrite.
+
+End Extra.
+
+Module interface.
+
+Export Core.
+
+Export Extra.
+
+End interface.
+
+Export interface.
+
