theories/SetModel/autosubst/AST_preamble.v
@@ -1,0 +1,3 @@
+From TypedConfluence Require Import core unscoped.
+From TypedConfluence Require Import BasicAST.
+From Stdlib Require Import Setoid Morphisms Relation_Definitions.
