theories/SetModel/model.v
@@ -7,7 +7,7 @@ Import ListNotations.
 Require Import library.
 Require Import ZF_axioms ZF_library ZF_nat ZF_acc.
 Require Import HO HO_univ HO_prop HO_box HO_pi HO_sigma HO_nat HO_obseq HO_forall.
-Require Import model_interp model_def model_univ model_pi model_nat.
+Require Import model_interp model_def model_univ model_pi model_nat model_acc.
 
 Open Scope subst_scope.
 
@@ -19,12 +19,12 @@ Combined Scheme ctx_typing_conversion_mutindS from typing_mutS, ctx_typing_mutS,
 (* Assumptions are validated by the model *)
 
 Lemma model_assm (Γ : ctx) (c : nat) (A : term) (tΓ : ⊢ Γ) (mΓ : model_ctx Γ) (Hc : nth_error assm_sig c = Some A)
-  (tA : ∙ ⊢< Ax BasicAST.prop > A : Sort BasicAST.prop) (mA : model_typing ∙ (Ax BasicAST.prop) A (Sort BasicAST.prop)) :
-  model_typing Γ BasicAST.prop (assm c) A.
+  (tA : ∙ ⊢< Ax prop > A : Sort prop) (mA : model_typing ∙ (Ax prop) A (Sort prop)) :
+  model_typing Γ prop (assm c) A.
 Proof.
   destruct mΓ as [ iΓ fΓ ]. destruct mA as [ iΓ' fΓ' iΩ fΩ iA fA vΩ vA ]. econstructor.
   * exact fΓ.
-  * assert (interp_tm Γ (Ax BasicAST.prop) A (fun _ => iA ∅)) as H. admit. exact H. (* weakening of interpretation *)
+  * assert (interp_tm Γ (Ax prop) A (fun _ => iA ∅)) as H. admit. exact H. (* weakening of interpretation *)
   * intros γ Hγ. cbn. inversion fΓ'. subst. inversion fΩ. subst.
     assert (∅ ∈ ⋆) as Hγ'. { now apply inSetSingl. } 
     refine (transpS (fun X => iA ∅ ∈ X) _ (vA _ Hγ')). now apply el_propTy.
@@ -48,10 +48,10 @@ Proof.
   - apply model_zero.
   - apply model_suc.
   - apply model_natrec.
-  - admit. (* apply model_acc *)
-  - admit. (* apply model_accin *)
-  - admit. (* apply model_accinv *)
-  - admit. (* apply model_accelim *)
+  - apply model_acc. 
+  - apply model_accin.
+  - apply model_accinv.
+  - apply model_accelim.
   - admit. (* apply model_obseq *)
   - admit. (* apply model_obsrefl *)
   - admit. (* apply model_J *)
@@ -63,7 +63,7 @@ Admitted.
 
 (* Corollary : the theory is consistent *)
 
-Corollary consistency : forall t , ∙ ⊢< BasicAST.prop > t : Pi (ty 0) BasicAST.prop (Sort BasicAST.prop) (var 0) -> False.
+Corollary consistency : forall t , ∙ ⊢< prop > t : Pi (ty 0) prop (Sort prop) (var 0) -> False.
 Proof.
   (* We interpret the judgment in our ZF model *)
   intros t H. apply model in H. destruct H as [ iΓ fΓ iA fA _ vt ].
@@ -77,7 +77,7 @@ Proof.
   inversion H4 ; subst ; clear H4. 
   (* We derive a contradiction *)
   assert (∅ ∈ ⋆) as Hγ. { now apply inSetSingl. }
-  specialize (vt _ Hγ). clear Hγ. apply prop_true_if in vt.
+  specialize (vt _ Hγ). clear Hγ. apply subsingl_true_if in vt.
   assert (∅ ∈ 𝕌el 0 (propTy_HO ∅)) as Hp.
   { refine (transpS (fun X => ∅ ∈ X) (sym el_propTy) _).
     apply ZFinpower. intros x Hx. apply ZFinempty in Hx. destruct Hx. }
