theories/SetModel/model_acc.v
@@ -1,0 +1,59 @@
+From Stdlib Require Import List Arith.
+From TypedConfluence Require Import core unscoped AST SubstNotations.
+From TypedConfluence Require Import Util BasicAST Contexts Typing. 
+
+Import ListNotations.
+Import CombineNotations.
+
+Require Import library.
+Require Import ZF_axioms ZF_library ZF_nat ZF_acc.
+Require Import HO HO_univ HO_prop HO_box HO_pi HO_sigma HO_nat HO_acc HO_obseq HO_forall.
+Require Import model_interp model_def.
+
+Lemma model_acc (Γ : ctx) (i : level) (A R a : term) (tA : Γ ⊢< Ax i > A : Sort i) (mA : model_typing Γ (Ax i) A (Sort i))
+  (tR : (Γ,, (i, A)),, (i, S ⋅ A) ⊢< Ax prop > R : Sort prop)
+  (mR : model_typing ((Γ,, (i, A)),, (i, S ⋅ A)) (Ax prop) R (Sort prop))
+  (ta : Γ ⊢< i > a : A) (ma : model_typing Γ i a A) :
+  model_typing Γ (Ax prop) (Core.acc i A R a) (Sort prop).
+Proof.
+Admitted.
+
+Lemma model_accin (Γ : ctx) (i : level) (A R a p : term) (tA : Γ ⊢< Ax i > A : Sort i) (mA : model_typing Γ (Ax i) A (Sort i))
+  (tR : (Γ,, (i, A)),, (i, S ⋅ A) ⊢< Ax prop > R : Sort prop)
+  (mR : model_typing ((Γ,, (i, A)),, (i, S ⋅ A)) (Ax prop) R (Sort prop))
+  (ta : Γ ⊢< i > a : A) (ma : model_typing Γ i a A)
+  (A_wk := (S >> S) ⋅ A)
+  (R_wk := (up_ren (up_ren (S >> S))) ⋅ R)
+  (acc_wk := Core.acc i A_wk R_wk (var 1))
+  (R' := R <[(S ⋅ a) .: (var 0 .: (S >> var))])
+  (tp : Γ ⊢< prop > p : Pi i prop A (Pi prop prop R' acc_wk))
+  (mp : model_typing Γ prop p (Pi i prop A (Pi prop prop R' acc_wk))) :
+  model_typing Γ prop (accin i A R a p) (Core.acc i A R a).
+Proof.
+Admitted.
+
+Lemma model_accinv (Γ : ctx) (i : level) (A R a p b r : term) (tA : Γ ⊢< Ax i > A : Sort i) (mA : model_typing Γ (Ax i) A (Sort i))
+  (tR : (Γ,, (i, A)),, (i, S ⋅ A) ⊢< Ax prop > R : Sort prop)
+  (mR : model_typing ((Γ,, (i, A)),, (i, S ⋅ A)) (Ax prop) R (Sort prop))
+  (ta : Γ ⊢< i > a : A) (ma : model_typing Γ i a A)
+  (tp : Γ ⊢< prop > p : Core.acc i A R a) (mp : model_typing Γ prop p (Core.acc i A R a))
+  (tb : Γ ⊢< i > b : A) (mb : model_typing Γ i b A)
+  (tr : Γ ⊢< prop > r : R <[ scons a b..]) (mr : model_typing Γ prop r (R <[ scons a b..])) :
+  model_typing Γ prop (accinv i A R a p b r) (Core.acc i A R b).
+Proof.
+Admitted.
+
+Lemma model_accelim (Γ : ctx) (i l : level) (A R a q P p : term) (tA : Γ ⊢< Ax i > A : Sort i) (mA : model_typing Γ (Ax i) A (Sort i))
+  (tR : (Γ,, (i, A)),, (i, S ⋅ A) ⊢< Ax prop > R : Sort prop)
+  (mR : model_typing ((Γ,, (i, A)),, (i, S ⋅ A)) (Ax prop) R (Sort prop))
+  (tP : Γ,, (i, A) ⊢< Ax l > P : Sort l) (mP : model_typing (Γ,, (i, A)) (Ax l) P (Sort l))
+  (R' := R <[var 1 .: (var 0 .: (S >> S >> var))])
+  (P' := P <[var 1 .: (S >> S >> S >> var)])
+  (B := Pi i l (S ⋅ A) (Pi prop l R' P'))
+  (P'' := P <[var 1.: (S >> (S >> var))])
+  (tp : (Γ,, (i, A)),, (Ru i l, B) ⊢< l > p : P'') (mp : model_typing ((Γ,, (i, A)),, (Ru i l, B)) l p P'')
+  (ta : Γ ⊢< i > a : A) (ma : model_typing Γ i a A)
+  (tq : Γ ⊢< prop > q : Core.acc i A R a) (mq : model_typing Γ prop q (Core.acc i A R a)) :
+  model_typing Γ l (accel i l A R P p a q) (P <[ a..]).
+Proof.
+Admitted.
