theories/SetModel/model_obseq.v
@@ -1,0 +1,33 @@
+From Stdlib Require Import List Arith.
+From TypedConfluence Require Import core unscoped AST SubstNotations.
+From TypedConfluence Require Import Util BasicAST Contexts Typing. 
+
+Import ListNotations.
+Import CombineNotations.
+
+Require Import library.
+Require Import ZF_axioms ZF_library ZF_nat ZF_acc.
+Require Import HO HO_univ HO_prop HO_box HO_pi HO_sigma HO_nat HO_acc HO_obseq HO_forall.
+Require Import model_interp model_def.
+
+Lemma model_obseq (Γ : ctx) (i : level) (A a b : term) (tA : Γ ⊢< Ax i > A : Sort i) (mA : model_typing Γ (Ax i) A (Sort i))
+  (ta : Γ ⊢< i > a : A) (ma : model_typing Γ i a A)
+  (tb : Γ ⊢< i > b : A) (mb : model_typing Γ i b A) :
+  model_typing Γ (Ax prop) (obseq i A a b) (Sort prop).
+Proof.
+  destruct i as [ i | ].
+  - destruct ma as [ iΓ fΓ iA fA ia fa vA va ]. destruct mb as [ iΓ' fΓ' iA' fA' ib fb vA' vb ].
+    destruct (functional_ctx Γ fΓ fΓ'). destruct (functional_tm A fA fA'). clear fΓ' fA' vA'. econstructor.
+    + exact fΓ.
+    + apply interp_prop.
+    + apply interp_obseq_r. exact fA. exact fa. exact fb.
+    + apply propTy_HO_typing.
+    + eapply eqTy_HO_typing'. exact vA. exact va. exact vb.
+  - destruct ma as [ iΓ fΓ iA fA vA va ]. destruct mb as [ iΓ' fΓ' iA' fA' vA' vb ].
+    destruct (functional_ctx Γ fΓ fΓ'). destruct (functional_tm A fA fA'). clear fΓ' fA' vA'. econstructor.
+    + exact fΓ.
+    + apply interp_prop.
+    + apply interp_obseq_i. 
+    + apply propTy_HO_typing.
+    + intros. refine (transpS (fun X => ⋆ ∈ X) (sym _) _). apply el_propTy. now apply ZFinpower. 
+Qed.
